Pushing hashtable proofs.

mailbox/verif_hashtable_atomic.v
@@ -1,6 +1,7 @@
 Require Import VST.veric.rmaps.
 Require Import VST.progs.ghosts.
 Require Import mailbox.general_atomics.
+Require Import mailbox.SC_atomics.
 Require Import VST.progs.conclib.
 Require Import mailbox.maps.
 Require Import VST.floyd.library.
@@ -13,6 +14,10 @@ Set Bullet Behavior "Strict Subproofs".
 Instance CompSpecs : compspecs. make_compspecs prog. Defined.
 Definition Vprog : varspecs. mk_varspecs prog. Defined.
 
+Section Proofs.
+
+Context {inv_names : invG}.
+
 Definition makelock_spec := DECLARE _makelock (makelock_spec _).
 Definition freelock2_spec := DECLARE _freelock2 (freelock2_spec _).
 Definition acquire_spec := DECLARE _acquire acquire_spec.
@@ -24,15 +29,16 @@ Definition CAS_SC_spec := DECLARE _CAS_SC CAS_SC_spec.
 
 Definition surely_malloc_spec :=
  DECLARE _surely_malloc
-   WITH n:Z
+   WITH t : type
    PRE [ _n OF tuint ]
-       PROP (0 <= n <= Int.max_unsigned)
-       LOCAL (temp _n (Vint (Int.repr n)))
+       PROP (0 <= sizeof t <= Int.max_unsigned; complete_legal_cosu_type t = true;
+             natural_aligned natural_alignment t = true)
+       LOCAL (temp _n (Vint (Int.repr (sizeof t))))
        SEP ()
     POST [ tptr tvoid ] EX p:_,
        PROP ()
        LOCAL (temp ret_temp p)
-       SEP (malloc_token Tsh n p * memory_block Tsh n p).
+       SEP (malloc_token Tsh t p * data_at_ Tsh t p).
 
 Definition integer_hash_spec :=
  DECLARE _integer_hash
@@ -59,11 +65,36 @@ Proof.
 Defined.
 
 (* We don't need histories, but we do need to know that a non-zero key is persistent. *)
-Instance zero_PCM : PCM Z := { join a b c := (a = 0 \/ a = c) /\ (b = 0 \/ b = c) }.
+Instance zero_PCM : Ghost := { valid a := True;
+  Join_G a b c := if eq_dec a 0 then c = b else c = a /\ (b = 0 \/ a = b) }.
 Proof.
-  - intros; tauto.
-  - intros.
-    exists e; destruct Hjoin1 as [[|][|]], Hjoin2 as [[|][|]]; subst; auto.
+  - exists (fun _ => 0); auto.
+    intro; hnf; auto.
+  - constructor.
+    + intros; hnf in *.
+      if_tac in H; subst; auto.
+      destruct H, H0; subst; auto.
+    + intros; hnf in *.
+      exists (if eq_dec b 0 then c else b); split; hnf.
+      * if_tac; auto; split; auto.
+        if_tac in H; subst.
+        { rewrite if_false in H0 by auto; tauto. }
+        destruct H as [? [|]]; try contradiction; subst.
+        rewrite if_false in H0 by auto; tauto.
+      * if_tac; subst.
+        { if_tac in H0; tauto. }
+        destruct H; subst.
+        if_tac; subst.
+        { if_tac in H0; subst; auto; contradiction. }
+        destruct H2; try contradiction; subst.
+        rewrite if_false in H0 by auto; tauto.
+    + intros; hnf in *.
+      if_tac; if_tac in H; subst; auto; try tauto.
+      destruct H as [? [|]]; subst; auto; contradiction.
+    + intros; hnf in *.
+      if_tac in H; if_tac in H0; subst; auto; try tauto.
+      destruct H; subst; contradiction.
+  - auto.
 Defined.
 
 Instance zero_order : PCM_order (fun a b => a = 0 \/ a = b).
@@ -71,42 +102,48 @@ Proof.
   constructor; simpl; intros.
   - intro; auto.
   - intros ???[|][|]; subst; auto.
-  - eauto.
-  - auto.
-  - auto.
+  - exists (if eq_dec a 0 then b else a).
+    unfold sepalg.join; simpl.
+    if_tac; auto.
+    destruct H; [contradiction|].
+    subst; repeat split; auto.
+    destruct H0; auto.
+  - hnf in H.
+    if_tac in H; auto.
+    destruct H; subst; split; auto.
+    destruct H1; auto.
+  - hnf.
+    if_tac; subst.
+    + destruct H; auto.
+    + split; auto; destruct H; auto.
 Defined.
 
 Definition hashtable_entry T lg entries i :=
-  let '(pk, pv) := Znth i entries (Vundef, Vundef) in let '(ki, vi) := Znth i T (0, 0) in
-  !!(repable_signed ki /\ repable_signed vi /\ (ki = 0 -> vi = 0)) && ghost_master ki (Znth i lg Vundef) *
+  let '(pk, pv) := Znth i entries in let '(ki, vi) := Znth i T in
+  !!(repable_signed ki /\ repable_signed vi /\ (ki = 0 -> vi = 0)) &&
+  ghost_master1(ORD := zero_order) ki (Znth i lg) *
   data_at Tsh tint (vint ki) pk * data_at Tsh tint (vint vi) pv.
 
-Definition wf_table T := forall k i, k <> 0 -> fst (Znth i T (0, 0)) = k -> lookup T k = Some i.
-
-Existing Instance exclusive_PCM.
+Definition wf_table T := forall k i, k <> 0 -> fst (Znth i T) = k -> lookup T k = Some i.
 
 Definition hashtable H g lg entries := EX T : list (Z * Z),
   !!(Zlength T = size /\ wf_table T /\ forall k v, H k = Some v <-> In (k, v) T /\ v <> 0) &&
-  ghost (Some H) g * fold_right sepcon emp (map (hashtable_entry T lg entries) (upto (Z.to_nat size))).
+  excl g H * fold_right sepcon emp (map (hashtable_entry T lg entries) (upto (Z.to_nat size))).
 
 Program Definition set_item_spec := DECLARE _set_item atomic_spec
-  (ConstType (Z * Z * val * share * list (val * val) * val * list val)) empty_map
+  (ConstType (Z * Z * globals * share * list (val * val) * gname * list gname))
   [(_key, tint); (_value, tint)] tvoid
-  [fun _ '(k, v, p, sh, entries, g, lg) => temp _key (vint k);
-   fun _ '(k, v, p, sh, entries, g, lg) => temp _value (vint v);
-   fun _ '(k, v, p, sh, entries, g, lg) => gvar _m_entries p]
-  (fun _ '(k, v, p, sh, entries, g, lg) => !!(readable_share sh /\ repable_signed k /\ repable_signed v /\
+  [fun _ '(k, v, gv, sh, entries, g, lg) => temp _key (vint k);
+   fun _ '(k, v, gv, sh, entries, g, lg) => temp _value (vint v);
+   fun _ '(k, v, gv, sh, entries, g, lg) => gvars gv]
+  (fun _ '(k, v, gv, sh, entries, g, lg) => !!(readable_share sh /\ repable_signed k /\ repable_signed v /\
    k <> 0 /\ v <> 0 /\ Forall (fun '(pk, pv) => isptr pk /\ isptr pv) entries /\ Zlength lg = size) &&
-   data_at sh (tarray tentry size) entries p)
-  (fun _ '(k, v, p, sh, entries, g, lg) H => hashtable H g lg entries)
+   data_at sh (tarray tentry size) entries (gv _m_entries))
+  (fun _ '(k, v, gv, sh, entries, g, lg) H => hashtable H g lg entries)
   tt []
-  (fun _ '(k, v, p, sh, entries, g, lg) _ _ => data_at sh (tarray tentry size) entries p)
-  (fun _ '(k, v, p, sh, entries, g, lg) H _ => hashtable (map_upd H k v) g lg entries)
-  _ _ _ _ _ _.
-Next Obligation.
-Proof.
-  intros ?? ((((((k, v), p), sh), entries), g), lg); auto.
-Qed.
+  (fun _ '(k, v, gv, sh, entries, g, lg) H _ =>
+   data_at sh (tarray tentry size) entries (gv _m_entries) * hashtable (map_upd H k v) g lg entries)
+  (Empty_set _) (Full_set _) _ _ _ _ _.
 Next Obligation.
 Proof.
   intros ?? ((((((k, v), p), sh), entries), g), lg); auto.
@@ -130,23 +167,18 @@ Qed.
 
 (* Read the most recently written value. *)
 Program Definition get_item_spec := DECLARE _get_item atomic_spec
-  (ConstType (Z * val * share * list (val * val) * val * list val)) empty_map
+  (ConstType (Z * globals * share * list (val * val) * gname * list gname))
   [(_key, tint)] tint
   [fun _ '(k, p, sh, entries, g, lg) => temp _key (vint k);
-   fun _ '(k, p, sh, entries, g, lg) => gvar _m_entries p]
-  (fun _ '(k, p, sh, entries, g, lg) => !!(readable_share sh /\ repable_signed k /\ k <> 0 /\
+   fun _ '(k, gv, sh, entries, g, lg) => gvars gv]
+  (fun _ '(k, gv, sh, entries, g, lg) => !!(readable_share sh /\ repable_signed k /\ k <> 0 /\
    Forall (fun '(pk, pv) => isptr pk /\ isptr pv) entries /\ Zlength lg = size) &&
-   data_at sh (tarray tentry size) entries p)
+   data_at sh (tarray tentry size) entries (gv _m_entries))
   (fun _ '(k, p, sh, entries, g, lg) H => hashtable H g lg entries)
   0 [fun _ _ v => temp ret_temp (vint v)]
-  (fun _ '(k, p, sh, entries, g, lg) _ _ => data_at sh (tarray tentry size) entries p)
-  (fun _ '(k, p, sh, entries, g, lg) H v => !!(if eq_dec v 0 then H k = None else H k = Some v) &&
-   hashtable H g lg entries)
-  _ _ _ _ _ _.
-Next Obligation.
-Proof.
-  intros ?? (((((k, p), sh), entries), g), lg); auto.
-Qed.
+  (fun _ '(k, gv, sh, entries, g, lg) H v => data_at sh (tarray tentry size) entries (gv _m_entries) *
+   (!!(if eq_dec v 0 then H k = None else H k = Some v) && hashtable H g lg entries))
+  (Empty_set _) (Full_set _) _ _ _ _ _.
 Next Obligation.
 Proof.
   intros ?? (((((k, p), sh), entries), g), lg); auto.
@@ -169,24 +201,19 @@ Proof.
 Qed.
 
 Program Definition add_item_spec := DECLARE _add_item atomic_spec
-  (ConstType (Z * Z * val * share * list (val * val) * val * list val)) empty_map
+  (ConstType (Z * Z * globals * share * list (val * val) * gname * list gname))
   [(_key, tint); (_value, tint)] tint
   [fun _ '(k, v, p, sh, entries, g, lg) => temp _key (vint k);
    fun _ '(k, v, p, sh, entries, g, lg) => temp _value (vint v);
-   fun _ '(k, v, p, sh, entries, g, lg) => gvar _m_entries p]
-  (fun _ '(k, v, p, sh, entries, g, lg) => !!(readable_share sh /\ repable_signed k /\ repable_signed v /\
+   fun _ '(k, v, gv, sh, entries, g, lg) => gvars gv]
+  (fun _ '(k, v, gv, sh, entries, g, lg) => !!(readable_share sh /\ repable_signed k /\ repable_signed v /\
    k <> 0 /\ v <> 0 /\ Forall (fun '(pk, pv) => isptr pk /\ isptr pv) entries /\ Zlength lg = size) &&
-   data_at sh (tarray tentry size) entries p)
+   data_at sh (tarray tentry size) entries (gv _m_entries))
   (fun _ '(k, v, p, sh, entries, g, lg) H => hashtable H g lg entries)
   true [fun _ _ b => temp ret_temp (Val.of_bool b)]
-  (fun _ '(k, v, p, sh, entries, g, lg) _ _ => data_at sh (tarray tentry size) entries p)
-  (fun _ '(k, v, p, sh, entries, g, lg) H b => !!(H k = None <-> b = true) &&
-   hashtable (if b then map_upd H k v else H) g lg entries)
-  _ _ _ _ _ _.
-Next Obligation.
-Proof.
-  intros ?? ((((((k, v), p), sh), entries), g), lg); auto.
-Qed.
+  (fun _ '(k, v, gv, sh, entries, g, lg) H b => data_at sh (tarray tentry size) entries (gv _m_entries) *
+   (!!(H k = None <-> b = true) && hashtable (if b then map_upd H k v else H) g lg entries))
+  (Empty_set _) (Full_set _) _ _ _ _ _.
 Next Obligation.
 Proof.
   intros ?? ((((((k, v), p), sh), entries), g), lg); auto.
@@ -210,20 +237,19 @@ Qed.
 
 Definition init_table_spec :=
  DECLARE _init_table
-  WITH p : val
+  WITH gv : globals
   PRE [ ]
    PROP ()
-   LOCAL (gvar _m_entries p)
-   SEP (data_at_ Ews (tarray tentry size) p)
+   LOCAL (gvars gv)
+   SEP (data_at_ Ews (tarray tentry size) (gv _m_entries))
   POST [ tvoid ]
-   EX entries : list (val * val), EX g : val, EX lg : list val,
+   EX entries : list (val * val), EX g : gname, EX lg : list gname,
    PROP (Forall (fun '(pk, pv) => isptr pk /\ isptr pv) entries; Zlength lg = size)
    LOCAL ()
-   SEP (data_at Ews (tarray tentry size) entries p; fold_right sepcon emp (map (fun '(pk, pv) =>
-          malloc_token Tsh (sizeof tint) pk * malloc_token Tsh (sizeof tint) pv) entries);
+   SEP (data_at Ews (tarray tentry size) entries (gv _m_entries); fold_right sepcon emp (map (fun '(pk, pv) =>
+          malloc_token Tsh tint pk * malloc_token Tsh tint pv) entries);
         hashtable empty_map g lg entries).
 
-(* Can we use this to relate atomicity to linearizability? *)
 Inductive hashtable_hist_el :=
   | HSet (k : Z) (v : Z) | HGet (k : Z) (v : Z) | HAdd (k : Z) (v : Z) (r : bool).
 
@@ -242,39 +268,42 @@ Fixpoint apply_hist H h :=
 Definition hashtable_inv gh g lg entries := EX H : _, hashtable H g lg entries *
   EX hr : _, !!(apply_hist empty_map hr = Some H) && ghost_ref hr gh.
 
-Definition f_lock_inv sh gsh entries gh g lg p t locksp lockt resultsp res :=
+Definition f_lock_inv sh gsh entries i gh g lg p t locksp lockt resultsp res :=
   EX b1 : bool, EX b2 : bool, EX b3 : bool, EX h : _,
-    !!(add_events [] [HAdd 1 1 b1; HAdd 2 1 b2; HAdd 3 1 b3] h) && ghost_hist gsh h gh *
-    data_at sh (tarray tentry size) entries p * invariant (hashtable_inv gh g lg entries) *
+    !!(add_events empty_map [HAdd 1 1 b1; HAdd 2 1 b2; HAdd 3 1 b3] h) && ghost_hist gsh h gh *
+    data_at sh (tarray tentry size) entries p * invariant i (hashtable_inv gh g lg entries) *
     data_at sh (tarray (tptr tlock) 3) (upd_Znth t (repeat Vundef 3) lockt) locksp *
     data_at sh (tarray (tptr tint) 3) (upd_Znth t (repeat Vundef 3) res) resultsp *
     data_at Tsh tint (vint (Zlength (filter id [b1; b2; b3]))) res.
 
-Definition f_lock_pred tsh sh gsh entries gh g lg p t locksp lockt resultsp res :=
-  selflock (f_lock_inv sh gsh entries gh g lg p t locksp lockt resultsp res) tsh lockt.
+Definition f_lock_pred tsh sh gsh entries i gh g lg p t locksp lockt resultsp res :=
+  selflock (f_lock_inv sh gsh entries i gh g lg p t locksp lockt resultsp res) tsh lockt.
 
 Definition f_spec :=
  DECLARE _f
-  WITH tid : val, x : share * share * share * list (val * val) * val * val * list val * val * Z * val *
+  WITH tid : val, x : share * share * share * list (val * val) * iname * gname * gname * list gname * globals * Z * val *
                       val * val * val
   PRE [ _arg OF (tptr tvoid) ]
-   let '(sh, gsh, tsh, entries, gh, g, lg, p, t, locksp, lockt, resultsp, res) := x in
+   let '(sh, gsh, tsh, entries, i, gh, g, lg, gv, t, locksp, lockt, resultsp, res) := x in
    PROP (0 <= t < 3; isptr lockt; readable_share sh; readable_share tsh; gsh <> Share.bot;
          Forall (fun '(pk, pv) => isptr pk /\ isptr pv) entries; Zlength lg = size)
-   LOCAL (temp _arg tid; gvar _m_entries p; gvar _thread_locks locksp; gvar _results resultsp)
-   SEP (data_at sh (tarray tentry size) entries p; invariant (hashtable_inv gh g lg entries);
-        ghost_hist gsh ([] : hist) gh; data_at Tsh tint (vint t) tid; malloc_token Tsh (sizeof tint) tid;
-        data_at sh (tarray (tptr tlock) 3) (upd_Znth t (repeat Vundef 3) lockt) locksp;
-        data_at sh (tarray (tptr tint) 3) (upd_Znth t (repeat Vundef 3) res) resultsp;
+   LOCAL (temp _arg tid; gvars gv)
+   SEP (data_at sh (tarray tentry size) entries (gv _m_entries);
+        invariant i (hashtable_inv gh g lg entries);
+        ghost_hist(hist_el := hashtable_hist_el) gsh empty_map gh;
+        data_at Tsh tint (vint t) tid; malloc_token Tsh tint tid;
+        data_at sh (tarray (tptr tlock) 3) (upd_Znth t (repeat Vundef 3) lockt) (gv _thread_locks);
+        data_at sh (tarray (tptr tint) 3) (upd_Znth t (repeat Vundef 3) res) (gv _results);
         data_at_ Tsh tint res;
-        lock_inv tsh lockt (f_lock_pred tsh sh gsh entries gh g lg p t locksp lockt resultsp res))
+        lock_inv tsh lockt (f_lock_pred tsh sh gsh entries i gh g lg (gv _m_entries) t
+                                        (gv _thread_locks) lockt (gv _results) res))
   POST [ tptr tvoid ] PROP () LOCAL () SEP ().
 
 Definition main_spec :=
  DECLARE _main
-  WITH u : unit
-  PRE  [] main_pre prog [] u
-  POST [ tint ] main_post prog [] u.
+  WITH gv : globals
+  PRE  [] main_pre prog [] gv
+  POST [ tint ] main_post prog [] gv.
 
 Definition Gprog : funspecs := ltac:(with_library prog [makelock_spec; freelock2_spec; acquire_spec;
   release2_spec; spawn_spec; surely_malloc_spec; load_SC_spec; store_SC_spec; CAS_SC_spec;
@@ -297,31 +326,19 @@ Qed.
 Arguments size : simpl never.
 Arguments hash : simpl never.
 
-(*Lemma forget_ghosts : forall (keys : list Z) lg, Zlength keys = Zlength lg ->
-  view_shift (fold_right sepcon emp (map (fun '(k', p) => ghost_snap k' p) (combine keys lg)))
-             (fold_right sepcon emp (map (ghost_snap 0) lg)).
-Proof.
-  induction keys; intros.
-  - symmetry in H; apply Zlength_nil_inv in H; subst; reflexivity.
-  - destruct lg; [apply Zlength_nil_inv in H; discriminate|].
-    rewrite !Zlength_cons in *; simpl.
-    apply view_shift_sepcon; [apply ghost_snap_forget; auto|].
-    apply IHkeys; omega.
-Qed.*)
-
 Lemma failed_entries : forall k i i1 keys lg T entries (Hk : k <> 0) (Hi : 0 <= i < size)
   (Hi1 : (i + hash k) mod size = i1 mod size) (HT : Zlength T = size) (Hlg : Zlength lg = size)
   (Hkeys: Zlength keys = size)
   (Hfail : Forall (fun z => z <> 0 /\ z <> k) (sublist 0 i (rebase keys (hash k)))),
   fold_right sepcon emp (upd_Znth (i1 mod size) (map (hashtable_entry T lg entries) (upto (Z.to_nat size))) emp) *
-  fold_right sepcon emp (map (fun i => ghost_snap (Znth ((i + hash k) mod size) keys 0)
-    (Znth ((i + hash k) mod size) lg Vundef)) (upto (Z.to_nat i)))
+  fold_right sepcon emp (map (fun i => ghost_snap (Znth ((i + hash k) mod size) keys)
+    (Znth ((i + hash k) mod size) lg)) (upto (Z.to_nat i)))
   |-- !! Forall (fun x => fst x <> 0 /\ fst x <> k) (sublist 0 i (rebase T (hash k))).
 Proof.
   intros.
   rewrite Forall_forall, prop_forall; apply allp_right; intros (k', v').
   rewrite prop_forall; apply allp_right; intro Hin.
-  apply In_Znth with (d := (0, 0)) in Hin; destruct Hin as (j & Hj & Hjth).
+  apply In_Znth in Hin; destruct Hin as (j & Hj & Hjth).
   pose proof (hash_range k).
   rewrite Zlength_sublist in Hj by (rewrite ?Zlength_rebase; omega).
   rewrite Znth_sublist, Znth_rebase in Hjth by omega.
@@ -337,11 +354,12 @@ Proof.
     (rewrite ?Zlength_map, ?Zlength_upto, ?Z2Nat.id; omega).
   unfold hashtable_entry.
   rewrite Z.add_0_r in Hjth; replace (Zlength T) with size in Hjth; rewrite Hjth.
-  destruct (Znth _ _ (Vundef, Vundef)).
-  Intros; rewrite <- !sepcon_assoc, (sepcon_comm _ (ghost_snap (Znth _ _ _) _)).
+  destruct (Znth _ entries).
+  Intros; rewrite <- !sepcon_assoc.
+  rewrite (sepcon_comm _ (ghost_snap(P := zero_PCM) _ _)).
   rewrite <- !sepcon_assoc, snap_master_join1 by auto.
   Intros; apply prop_right; simpl.
-  eapply Forall_Znth with (d := 0) in Hfail.
+  eapply Forall_Znth in Hfail.
   rewrite Znth_sublist, Z.add_0_r, Znth_rebase with (i0 := j) in Hfail; auto; try omega.
   replace (Zlength keys) with size in Hfail; intuition.
   { rewrite Zlength_sublist; auto; try omega.
@@ -352,10 +370,10 @@ Corollary entries_lookup : forall k i i1 keys lg T entries (Hk : k <> 0) (Hi : 0
   (Hi1 : (i + hash k) mod size = i1 mod size) (HT : Zlength T = size) (Hlg : Zlength lg = size)
   (Hkeys: Zlength keys = size)
   (Hfail : Forall (fun z => z <> 0 /\ z <> k) (sublist 0 i (rebase keys (hash k))))
-  (Hhit : fst (Znth (i1 mod size) T (0, 0)) = k \/ fst (Znth (i1 mod size) T (0, 0)) = 0),
+  (Hhit : fst (Znth (i1 mod size) T) = k \/ fst (Znth (i1 mod size) T) = 0),
   fold_right sepcon emp (upd_Znth (i1 mod size) (map (hashtable_entry T lg entries) (upto (Z.to_nat size))) emp) *
-  fold_right sepcon emp (map (fun i => ghost_snap (Znth ((i + hash k) mod size) keys 0)
-    (Znth ((i + hash k) mod size) lg Vundef)) (upto (Z.to_nat i)))
+  fold_right sepcon emp (map (fun i => ghost_snap (Znth ((i + hash k) mod size) keys)
+    (Znth ((i + hash k) mod size) lg)) (upto (Z.to_nat i)))
   |-- !! (lookup T k = Some (i1 mod size)).
 Proof.
   intros.
@@ -377,7 +395,7 @@ Proof.
   destruct (eq_dec i0 i); subst.
   - rewrite upd_Znth_same, lookup_upd_same; auto.
   - rewrite upd_Znth_diff' in Hj |- * by auto.
-    assert (lookup T (fst (Znth i0 T (0, 0))) <> Some i).
+    assert (lookup T (fst (Znth i0 T)) <> Some i).
     { erewrite Hwf by eauto; congruence. }
     rewrite lookup_upd_diff; auto.
     split; auto.
@@ -385,82 +403,115 @@ Proof.
 Qed.
 
 Corollary wf_table_upd_same : forall T k v i (Hwf : wf_table T) (HT : Zlength T = size)
-  (Hi : fst (Znth i T (0, 0)) = k) (Hk : k <> 0), wf_table (upd_Znth i T (k, v)).
+  (Hi : fst (Znth i T) = k) (Hk : k <> 0), wf_table (upd_Znth i T (k, v)).
 Proof.
   intros; apply wf_table_upd; auto.
+Qed.
+
+Lemma snaps_dealloc : forall {A} (l : list A) f g, fold_right sepcon emp (map (fun i => ghost_snap (f i) (g i)) l) |-- |==> emp.
+Proof.
+  induction l; simpl; intros.
+  - apply bupd_intro.
+  - eapply derives_trans; [apply sepcon_derives; [apply own_dealloc | apply IHl]|].
+    setoid_rewrite <- emp_sepcon at 7; apply bupd_sepcon.
 Qed.
 
 Lemma body_set_item : semax_body Vprog Gprog f_set_item set_item_spec.
 Proof.
   start_atomic_function.
-  destruct x as ((((((k, v), p), sh), entries), g), lg); Intros.
-  destruct H as (HP & HQ).
+  destruct x as ((((((k, v), gv), sh), entries), g), lg); Intros.
   forward_call k.
   pose proof size_pos.
-  eapply semax_pre with (P' := EX i : Z, EX i1 : Z, EX keys : list Z,
+  unfold atomic_shift; Intros P.
+  set (AS := weak_fview_shift _ _ _ _).
+  forward_loop (EX i : Z, EX i1 : Z, EX keys : list Z,
     PROP (i1 mod size = (i + hash k) mod size; 0 <= i < size; Zlength keys = size;
           Forall (fun z => z <> 0 /\ z <> k) (sublist 0 i (rebase keys (hash k))))
-    LOCAL (temp _idx (vint i1); temp _key (vint k); temp _value (vint v); gvar _m_entries p)
-    SEP (@data_at CompSpecs sh (tarray tentry size) entries p;
-         fold_right sepcon emp (map (fun i => ghost_snap (Znth ((i + hash k) mod size) keys 0)
-           (Znth ((i + hash k) mod size) lg Vundef)) (upto (Z.to_nat i)));
-         fold_right sepcon emp (map (fun p0 => invariant (II p0)) lI); P)).
+    LOCAL (temp _idx (vint i1); temp _key (vint k); temp _value (vint v); gvars gv)
+    SEP (|> P; AS && emp;
+         @data_at CompSpecs sh (tarray tentry size) entries (gv _m_entries);
+         fold_right sepcon emp (map (fun i => ghost_snap (Znth ((i + hash k) mod size) keys)
+           (Znth ((i + hash k) mod size) lg)) (upto (Z.to_nat i)))))%assert
+    continue: (EX i : Z, EX i1 : Z, EX keys : list Z,
+    PROP (Int.min_signed <= Int.signed (Int.repr i1) < Int.max_signed; i1 mod size = (i + hash k) mod size;
+          0 <= i < size; Zlength keys = size;
+          Forall (fun z => z <> 0 /\ z <> k) (sublist 0 (i + 1) (rebase keys (hash k))))
+    LOCAL (temp _idx (vint i1); temp _key (vint k); temp _value (vint v); gvars gv)
+    SEP (|> P; AS && emp; @data_at CompSpecs sh (tarray tentry size) entries (gv _m_entries);
+         fold_right sepcon emp (map (fun i => ghost_snap (Znth ((i + hash k) mod size) keys)
+           (Znth ((i + hash k) mod size) lg)) (upto (Z.to_nat (i + 1))))))%assert.
   { Exists 0 (k * 654435761)%Z (repeat 0 (Z.to_nat size)); rewrite sublist_nil; entailer!.
     split; [apply hash_size|].
-    rewrite Zlength_repeat, Z2Nat.id; auto; omega. }
-  eapply semax_loop.
+    rewrite Zlength_repeat, Z2Nat.id; auto; omega.
+    { simpl; auto. } }
   - Intros i i1 keys; forward.
-    forward.
     rewrite sub_repr, and_repr; simpl.
     rewrite Zland_two_p with (n := 14) by omega.
     replace (2 ^ 14) with size by (setoid_rewrite (proj2_sig has_size); auto).
     exploit (Z_mod_lt i1 size); [omega | intro Hi1].
     assert_PROP (Zlength entries = size) as Hentries by entailer!.
     assert (0 <= i1 mod size < Zlength entries) as Hi1' by omega.
-    match goal with H : Forall _ _ |- _ => pose proof (Forall_Znth _ _ _ (Vundef, Vundef) Hi1' H) as Hptr end.
-    destruct (Znth (i1 mod size) entries (Vundef, Vundef)) as (pki, pvi) eqn: Hpi; destruct Hptr.
-    forward; rewrite Hpi.
+    match goal with H : Forall _ _ |- _ => pose proof (Forall_Znth _ _ _ Hi1' H) as Hptr end.
+    destruct (Znth (i1 mod size) entries) as (pki, pvi) eqn: Hpi; destruct Hptr.
+    forward; setoid_rewrite Hpi.
     { entailer!. }
     assert (Zlength (rebase keys (hash k)) = size) as Hrebase.
     { rewrite Zlength_rebase; replace (Zlength keys) with size; auto; apply hash_range. }
-    forward_call (pki, P, II, lI,
+    forward_call (pki, AS && emp * |> P, Full_set iname, Empty_set iname,
       fun sh v => !!(sh = Tsh) && EX H : _, EX T : _, !!(Zlength T = size /\ wf_table T /\
-      forall k v, H k = Some v <-> In (k, v) T /\ v <> 0) && let '(ki, vi) := Znth (i1 mod size) T (0, 0) in
-      !!(v = ki /\ repable_signed vi /\ (ki = 0 -> vi = 0)) && ghost_master ki (Znth (i1 mod size) lg Vundef) *
-      data_at Tsh tint (vint vi) pvi * ghost (Some H) g * fold_right sepcon emp (upd_Znth (i1 mod size)
-          (map (hashtable_entry T lg entries) (upto (Z.to_nat size))) emp) * R H,
-      fun v : Z => P * ghost_snap v (Znth (i1 mod size) lg Vundef)).
-    { split.
-      + etransitivity; [apply HP|].
-        view_shift_intro HT.
-        apply derives_view_shift.
-        unfold hashtable; Intros T.
+      forall k v, H k = Some v <-> In (k, v) T /\ v <> 0) && let '(ki, vi) := Znth (i1 mod size) T in
+      !!(v = ki /\ repable_signed vi /\ (ki = 0 -> vi = 0)) && ghost_master1 ki (Znth (i1 mod size) lg) *
+      data_at Tsh tint (vint vi) pvi * excl g H * fold_right sepcon emp (upd_Znth (i1 mod size)
+          (map (hashtable_entry T lg entries) (upto (Z.to_nat size))) emp) *
+      (weak_fview_shift (Empty_set iname) (Full_set iname) (hashtable H g lg entries) (|> P) && emp),
+      fun v : Z => |> P * ghost_snap v (Znth (i1 mod size) lg)).
+    { rewrite emp_dup at 1; cancel.
+      rewrite <- emp_sepcon at 1; apply sepcon_derives; [|cancel].
+      rewrite <- emp_sepcon at 1; apply sepcon_derives.
+      + unfold weak_fview_shift; rewrite <- wand_sepcon_adjoint, emp_sepcon.
+        unfold AS.
+        eapply derives_trans; [apply apply_fview_shift|].
+        apply fupd_mono.
+        Intros HT.
+        unfold hashtable at 1; Intros T.
         rewrite extract_nth_sepcon with (i := i1 mod size)
           by (rewrite Zlength_map, Zlength_upto, Z2Nat.id; omega).
         erewrite Znth_map, Znth_upto by (rewrite ?Zlength_upto, Z2Nat.id; omega).
         unfold hashtable_entry.
         rewrite Hpi.
-        destruct (Znth (i1 mod size) T (0, 0)) as (ki, vi) eqn: HHi.
+        destruct (Znth (i1 mod size) T) as (ki, vi) eqn: HHi.
+        eapply derives_trans; [apply sepcon_derives, andp_left1; apply derives_refl|].
         Intros; Exists Tsh ki HT T; rewrite HHi; entailer!.
-      + intros.
-        rewrite <- sepcon_assoc; etransitivity; [|apply view_shift_sepcon1, HP].
-        view_shift_intro HT.
-        view_shift_intro T.
-        destruct (Znth (i1 mod size) T (0, 0)) as (ki, vi) eqn: HHi; view_shift_intros.
-        rewrite <- !sepcon_assoc, (sepcon_comm _ (ghost_master _ _)).
-        rewrite !sepcon_assoc; etransitivity; [apply view_shift_sepcon1, make_snap|].
-        apply derives_view_shift.
-        Exists HT.
-        unfold hashtable; Exists T.
-        rewrite extract_nth_sepcon with (i := i1 mod size)(l := map _ _)
-          by (rewrite Zlength_map, Zlength_upto, Z2Nat.id; omega).
-        erewrite Znth_map, Znth_upto by (rewrite ?Zlength_upto, Z2Nat.id; omega).
-        unfold hashtable_entry.
-        rewrite Hpi, HHi; entailer!. }
+        apply derives_refl.
+      + apply allp_right; intro sh0.
+        apply allp_right; intro v0.
+        unfold weak_fview_shift; rewrite <- wand_sepcon_adjoint, emp_sepcon.
+        Intros HT T.
+        destruct (Znth (i1 mod size) T) as (ki, vi) eqn: HHi; Intros.
+        rewrite <- !sepcon_assoc, (sepcon_comm _ (ghost_master1 _ _)).
+        rewrite !sepcon_assoc; eapply derives_trans.
+        { apply sepcon_derives, derives_refl.
+          apply (make_snap(ORD := zero_order)). }
+        eapply derives_trans; [apply bupd_frame_r|].
+        apply fupd_bupd, bupd_mono.
+        eapply derives_trans.
+        { rewrite sepcon_assoc; apply sepcon_derives; [apply derives_refl|].
+          rewrite <- !sepcon_assoc, sepcon_comm.
+          eapply derives_trans, apply_fview_shift.
+          apply sepcon_derives; [apply derives_refl|].
+          unfold hashtable; Exists T.
+          rewrite extract_nth_sepcon with (i := i1 mod size)(l := map _ _)
+            by (rewrite Zlength_map, Zlength_upto, Z2Nat.id; omega).
+          erewrite Znth_map, Znth_upto by (rewrite ?Zlength_upto, Z2Nat.id; omega).
+          unfold hashtable_entry.
+          rewrite Hpi, HHi; entailer!.
+          apply derives_refl. }
+        eapply derives_trans; [apply fupd_frame_l|].
+        subst; apply fupd_mono; cancel. }
     Intros k1.
-    focus_SEP 2.
+    focus_SEP 1.
     match goal with |- semax _ (PROP () (LOCALx (_ :: ?Q) (SEPx (_ :: ?R)))) _ _ =>
-      forward_if (PROP () (LOCALx Q (SEPx (ghost_snap k (Znth (i1 mod size) lg Vundef) :: R)))) end.
+      forward_if (PROP () (LOCALx Q (SEPx (ghost_snap k (Znth (i1 mod size) lg) :: R)))) end.
     + assert (forall k1, (k1 <> k /\ k1 <> 0) ->
         Zlength (upd_Znth (i1 mod size) keys k1) = size /\
         Forall (fun z => z <> 0 /\ z <> k)
@@ -469,32 +520,26 @@ Proof.
         replace (i1 mod size) with ((i + hash k) mod size); replace size with (Zlength keys);
           rewrite !rebase_upd' by (try omega; replace (Zlength keys) with size; apply Z_mod_lt; omega).
         rewrite sublist_upd_Znth_lr by (try omega; setoid_rewrite Hrebase; omega).
-        rewrite sublist_split with (mid := i), sublist_len_1 with (d := 0) by (try omega; setoid_rewrite Hrebase; omega).
+        rewrite sublist_split with (mid := i), sublist_len_1 by (try omega; setoid_rewrite Hrebase; omega).
         rewrite Z.sub_0_r, upd_Znth_app2, Forall_app; rewrite Zlength_sublist;
           rewrite ?Zlength_cons, ?Zlength_nil; try omega; try (setoid_rewrite Hrebase; omega).
         split; auto.
         rewrite Z.sub_0_r, Zminus_diag, upd_Znth0, Zlength_cons, sublist_1_cons, sublist_same
           by (auto; omega).
         repeat constructor; auto; tauto. }
-      match goal with |- semax _ (PROP () (LOCALx ?Q (SEPx ?R))) _ _ =>
-        forward_if (PROP (k1 = 0) (LOCALx Q (SEPx R))) end.
+      forward_if (k1 = 0).
       { eapply semax_pre; [|apply semax_continue].
-        unfold POSTCONDITION, abbreviate, overridePost.
-        destruct (eq_dec EK_continue EK_normal); [discriminate|].
-        unfold loop1_ret_assert.
-        instantiate (1 := EX i : Z, EX i1 : Z, EX keys : list Z,
-          PROP (i1 mod size = (i + hash k) mod size; 0 <= i < size; Zlength keys = size;
-            Forall (fun z => z <> 0 /\ z <> k) (sublist 0 (i + 1) (rebase keys (hash k))))
-          LOCAL (temp _idx (vint i1); temp _key (vint k); temp _value (vint v); gvar _m_entries p)
-          SEP (@data_at CompSpecs sh (tarray tentry size) entries p;
-               fold_right sepcon emp (map (fun i => ghost_snap (Znth ((i + hash k) mod size) keys 0)
-                 (Znth ((i + hash k) mod size) lg Vundef)) (upto (Z.to_nat (i + 1))));
-               fold_right sepcon emp (map (fun p0 => invariant (II p0)) lI); P)).
+        unfold POSTCONDITION, abbreviate, overridePost, loop1_ret_assert, frame_ret_assert,
+          function_body_ret_assert, RA_continue.
         Exists i (i1 mod size) (upd_Znth (i1 mod size) keys k1).
         rewrite Z2Nat.inj_add, upto_app, map_app, sepcon_app by omega.
         change (upto (Z.to_nat 1)) with [0]; simpl fold_right; rewrite Z2Nat.id, Z.add_0_r by omega.
         replace ((i + hash k) mod size) with (i1 mod size); rewrite Zmod_mod, upd_Znth_same by omega; entailer!.
-        erewrite map_ext_in; eauto; simpl; intros.
+        { assert (Int.min_signed <= i1 mod size < Int.max_signed).
+          { split; etransitivity; try apply Z_mod_lt; auto; try computable.
+            setoid_rewrite (proj2_sig has_size); computable. }
+          rewrite Int.signed_repr by omega; auto. }
+        erewrite map_ext_in; [apply derives_refl|]; simpl; intros.
         rewrite upd_Znth_diff'; auto; try omega.
         replace (i1 mod size) with ((i + hash k) mod size); intro X; apply Zmod_plus_inv in X; auto.
         rewrite In_upto, Z2Nat.id in * by omega.
@@ -502,56 +547,70 @@ Proof.
       { forward.
         entailer!. }
       Intros; subst.
-      forward_call (pki, 0, k, P * ghost_snap 0 (Znth (i1 mod size) lg Vundef) *
-          fold_right sepcon emp (map (fun i => ghost_snap (Znth ((i + hash k) mod size) keys 0)
-             (Znth ((i + hash k) mod size) lg Vundef)) (upto (Z.to_nat i))),
-        II, lI, fun sh v => !!(sh = Tsh) && EX H : _, EX T : _, !!(Zlength T = size /\ wf_table T /\
-          forall k v, H k = Some v <-> In (k, v) T /\ v <> 0) && let '(ki, vi) := Znth (i1 mod size) T (0, 0) in
+      forward_call (pki, 0, k, |> P * (AS && emp) * ghost_snap 0 (Znth (i1 mod size) lg) *
+          fold_right sepcon emp (map (fun i => ghost_snap (Znth ((i + hash k) mod size) keys)
+             (Znth ((i + hash k) mod size) lg)) (upto (Z.to_nat i))),
+        Full_set iname, Empty_set iname, fun sh v => !!(sh = Tsh) && EX H : _, EX T : _, !!(Zlength T = size /\ wf_table T /\
+          forall k v, H k = Some v <-> In (k, v) T /\ v <> 0) && let '(ki, vi) := Znth (i1 mod size) T in
           !!(v = ki /\ repable_signed vi /\ (ki = 0 -> vi = 0)) &&
-          ghost_master ki (Znth (i1 mod size) lg Vundef) * data_at Tsh tint (vint vi) pvi *
-          ghost (Some H) g * fold_right sepcon emp (upd_Znth (i1 mod size)
+          ghost_master1 ki (Znth (i1 mod size) lg) * data_at Tsh tint (vint vi) pvi *
+          excl g H * fold_right sepcon emp (upd_Znth (i1 mod size)
             (map (hashtable_entry T lg entries) (upto (Z.to_nat size))) emp) *
-          R H * ghost_snap 0 (Znth (i1 mod size) lg Vundef) *
-          fold_right sepcon emp (map (fun i => ghost_snap (Znth ((i + hash k) mod size) keys 0)
-             (Znth ((i + hash k) mod size) lg Vundef)) (upto (Z.to_nat i))),
-        fun v : Z => P * ghost_snap (if eq_dec v 0 then k else v) (Znth (i1 mod size) lg Vundef) *
-          fold_right sepcon emp (map (fun i => ghost_snap (Znth ((i + hash k) mod size) keys 0)
-             (Znth ((i + hash k) mod size) lg Vundef)) (upto (Z.to_nat i)))).
-      { repeat (split; auto).
-        * rewrite <- !sepcon_assoc, sepcon_assoc; etransitivity; [apply view_shift_sepcon1, HP|].
-          view_shift_intro HT.
-          apply derives_view_shift.
-          unfold hashtable; Intros T.
+          ghost_snap 0 (Znth (i1 mod size) lg) *
+          fold_right sepcon emp (map (fun i => ghost_snap (Znth ((i + hash k) mod size) keys)
+             (Znth ((i + hash k) mod size) lg)) (upto (Z.to_nat i))) *
+          (weak_fview_shift (Empty_set _) (Full_set _) (hashtable H g lg entries) (|> P) && emp),
+        fun v : Z => |> P * ghost_snap (if eq_dec v 0 then k else v) (Znth (i1 mod size) lg) *
+          fold_right sepcon emp (map (fun i => ghost_snap (Znth ((i + hash k) mod size) keys)
+             (Znth ((i + hash k) mod size) lg)) (upto (Z.to_nat i)))).
+      { rewrite emp_dup at 1; cancel.
+        rewrite sepcon_comm, <- emp_sepcon at 1.
+        rewrite <- sepcon_assoc.
+        apply sepcon_derives; [|cancel]; apply sepcon_derives, derives_refl.
+        rewrite <- emp_sepcon at 1; apply sepcon_derives.
+        * unfold weak_fview_shift; rewrite <- wand_sepcon_adjoint, emp_sepcon.
+          rewrite sepcon_assoc, (sepcon_comm _ (AS && emp)); unfold AS.
+          eapply derives_trans; [apply sepcon_derives, derives_refl; apply apply_fview_shift|].
+          eapply derives_trans; [apply fupd_frame_r | apply fupd_mono].
+          Intros HT.
+          unfold hashtable at 1; Intros T.
           rewrite extract_nth_sepcon with (i := i1 mod size) by (rewrite Zlength_map, Zlength_upto, Z2Nat.id; omega).
           erewrite Znth_map, Znth_upto by (rewrite ?Zlength_upto, Z2Nat.id; omega).
           unfold hashtable_entry.
           rewrite Hpi.
-          destruct (Znth (i1 mod size) T (0, 0)) as (ki, vi) eqn: HHi.
-          Exists Tsh ki HT T; rewrite HHi; entailer!.
-        * intros.
-          rewrite <- !sepcon_assoc, sepcon_assoc; etransitivity; [|apply view_shift_sepcon1, HP].
-          view_shift_intro HT; view_shift_intro T.
-          destruct (Znth (i1 mod size) T (0, 0)) as (ki, vi) eqn: HHi.
-          view_shift_intros.
+          destruct (Znth (i1 mod size) T) as (ki, vi) eqn: HHi.
+          rewrite <- !sepcon_assoc, (sepcon_comm _ (_ && _)), !sepcon_assoc.
+          eapply derives_trans; [apply sepcon_derives; [apply andp_left1|]; apply derives_refl|].
+          Exists Tsh ki HT T; rewrite HHi; unfold weak_fview_shift; entailer!.
+          apply derives_refl.
+        * apply allp_right; intro sh0.
+          apply allp_right; intro v0.
+          unfold weak_fview_shift; rewrite <- wand_sepcon_adjoint, emp_sepcon.
+          Intros HT T.
+          destruct (Znth (i1 mod size) T) as (ki, vi) eqn: HHi; Intros.
           assert (0 <= i1 mod size < Zlength T) by omega.
-          rewrite <- !sepcon_assoc, (sepcon_comm _ (ghost_master _ _)).
+          rewrite <- !sepcon_assoc, (sepcon_comm _ (ghost_master1 _ _)).
           rewrite (sepcon_comm _ (ghost_snap _ _)), <- !sepcon_assoc.
-          rewrite 5sepcon_assoc; etransitivity; [apply view_shift_sepcon1|].
+          rewrite 5sepcon_assoc; eapply derives_trans; [apply sepcon_derives, derives_refl|].
           { apply snap_master_update1 with (v' := if eq_dec ki 0 then k else ki).
             if_tac; auto. }
-          apply derives_view_shift.
+          eapply derives_trans; [apply bupd_frame_r | apply fupd_bupd, bupd_mono].
           assert (0 <= hash k < Zlength T) by (replace (Zlength T) with size; apply hash_range).
           assert (0 <= i < Zlength (rebase T (hash k))) by (rewrite Zlength_rebase; auto; omega).
-          assert (fst (Znth i (rebase T (hash k)) (0, 0)) = ki).
+          assert (fst (Znth i (rebase T (hash k))) = ki).
           { rewrite Znth_rebase by (auto; omega).
             replace (Zlength T) with size; replace ((i + hash k) mod size) with (i1 mod size); rewrite HHi; auto. }
           assert_PROP ((ki = k \/ ki = 0) -> lookup T k = Some (i1 mod size)) as Hindex.
           { rewrite prop_forall; apply allp_right; intro Hki.
-            pose proof (entries_lookup k i i1 keys lg T entries) as Hlookup.
-            sep_apply Hlookup; auto.
-            { rewrite HHi; destruct Hki; subst; auto. }
-            apply sepcon_derives_prop; auto. }
-          Exists HT.
+            rewrite <- 3sepcon_assoc, sepcon_comm.
+            rewrite <- !sepcon_assoc, 5sepcon_assoc.
+            apply sepcon_derives_prop, entries_lookup; auto.
+            rewrite HHi; destruct Hki; subst; auto. }
+          rewrite !sepcon_assoc; eapply derives_trans, fupd_frame_r; subst v0; cancel.
+          rewrite !sepcon_assoc, sepcon_comm; apply sepcon_derives, derives_refl.
+          rewrite <- !sepcon_assoc, sepcon_comm.
+          eapply derives_trans, apply_fview_shift.
+          apply sepcon_derives; [apply derives_refl|].
           unfold hashtable; Exists (upd_Znth (i1 mod size) T (if eq_dec ki 0 then k else ki, vi)).
           rewrite extract_nth_sepcon with (i := i1 mod size)(l := map _ (upto (Z.to_nat size)))
             by (rewrite Zlength_map, Zlength_upto, Z2Nat.id; omega).
@@ -567,6 +626,7 @@ Proof.
             - eapply In_upd_Znth_old; auto; try omega.
               rewrite HHi; intro X; inv X; tauto.
             - apply In_upd_Znth in Hin; destruct Hin as [X|]; [inv X; tauto | auto]. }
+          apply sepcon_derives; [apply derives_refl|].
           apply sepcon_list_derives; rewrite !upd_Znth_Zlength;
             rewrite !Zlength_map, !Zlength_upto, !Z2Nat.id; auto; try omega.
           intros; destruct (eq_dec i0 (i1 mod size)).
@@ -575,130 +635,155 @@ Proof.
           erewrite !Znth_map, !Znth_upto by (rewrite ?Zlength_upto, Z2Nat.id; auto; omega).
           rewrite upd_Znth_diff'; auto. }
       Intros k1.
-      focus_SEP 2.
+      focus_SEP 1.
       match goal with |- semax _ (PROP () (LOCALx (_ :: _ :: ?Q) (SEPx (_ :: ?R)))) _ _ =>
-        forward_if (PROP () ((LOCALx Q) (SEPx (ghost_snap k (Znth (i1 mod size) lg Vundef) :: R)))) end.
+        forward_if (PROP () ((LOCALx Q) (SEPx (ghost_snap k (Znth (i1 mod size) lg) :: R)))) end.
       * if_tac; [discriminate|].
-        forward_call (pki, P * ghost_snap k1 (Znth (i1 mod size) lg Vundef), II, lI,
+        forward_call (pki, |> P * (AS && emp) * ghost_snap k1 (Znth (i1 mod size) lg), Full_set iname, Empty_set iname,
           fun sh v => !!(sh = Tsh) && EX H : _, EX T : _, !!(Zlength T = size /\ wf_table T /\
-            forall k v, H k = Some v <-> In (k, v) T /\ v <> 0) && let '(ki, vi) := Znth (i1 mod size) T (0, 0) in
+            forall k v, H k = Some v <-> In (k, v) T /\ v <> 0) && let '(ki, vi) := Znth (i1 mod size) T in
             !!(v = ki /\ repable_signed vi /\ (ki = 0 -> vi = 0)) &&
-            ghost_master ki (Znth (i1 mod size) lg Vundef) * data_at Tsh tint (vint vi) pvi *
-            ghost (Some H) g * fold_right sepcon emp (upd_Znth (i1 mod size)
+            ghost_master1 ki (Znth (i1 mod size) lg) * data_at Tsh tint (vint vi) pvi *
+            excl g H * fold_right sepcon emp (upd_Znth (i1 mod size)
               (map (hashtable_entry T lg entries) (upto (Z.to_nat size))) emp) *
-            R H * ghost_snap k1 (Znth (i1 mod size) lg Vundef),
-          fun v : Z => P * (!!(v = k1) && ghost_snap k1 (Znth (i1 mod size) lg Vundef))).
-        { split.
-          + rewrite <- sepcon_assoc; etransitivity; [apply view_shift_sepcon; [apply HP | reflexivity]|].
-            view_shift_intro HT.
-            apply derives_view_shift.
-            unfold hashtable; Intros T.
+            ghost_snap k1 (Znth (i1 mod size) lg) *
+            (weak_fview_shift (Empty_set _) (Full_set _) (hashtable H g lg entries) (|> P) && emp),
+          fun v : Z => |> P * (!!(v = k1) && ghost_snap k1 (Znth (i1 mod size) lg))).
+        { rewrite emp_dup at 1; cancel.
+          rewrite <- emp_sepcon at 1; apply sepcon_derives; [|cancel].
+          rewrite <- emp_sepcon at 1; apply sepcon_derives.
+          + unfold weak_fview_shift; rewrite <- wand_sepcon_adjoint, emp_sepcon.
+            rewrite (sepcon_comm _ (AS && emp)); unfold AS.
+            eapply derives_trans; [apply sepcon_derives, derives_refl; apply apply_fview_shift|].
+            eapply derives_trans; [apply fupd_frame_r | apply fupd_mono].
+            Intros HT.
+            unfold hashtable at 1; Intros T.
             rewrite extract_nth_sepcon with (i := i1 mod size)
               by (rewrite Zlength_map, Zlength_upto, Z2Nat.id; omega).
             erewrite Znth_map, Znth_upto by (rewrite ?Zlength_upto, Z2Nat.id; omega).
             unfold hashtable_entry.
             rewrite Hpi.
-            destruct (Znth (i1 mod size) T (0, 0)) as (ki, vi) eqn: HHi.
+            destruct (Znth (i1 mod size) T) as (ki, vi) eqn: HHi.
+            rewrite <- !sepcon_assoc, (sepcon_comm _ (_ && _)), !sepcon_assoc.
+            eapply derives_trans; [apply sepcon_derives; [apply andp_left1|]; apply derives_refl|].
             Exists Tsh ki HT T; rewrite HHi; entailer!.
-          + intros.
-            rewrite <- sepcon_assoc; etransitivity; [|apply view_shift_sepcon; [apply HP | reflexivity]].
-            view_shift_intro HT; view_shift_intro T.
-            destruct (Znth (i1 mod size) T (0, 0)) as (ki, vi) eqn: HHi.
-            view_shift_intros.
-            rewrite <- !sepcon_assoc, (sepcon_comm _ (ghost_master _ _)).
+            apply derives_refl.
+          + apply allp_right; intro sh0.
+            apply allp_right; intro v0.
+            unfold weak_fview_shift; rewrite <- wand_sepcon_adjoint, emp_sepcon.
+            Intros HT T.
+            destruct (Znth (i1 mod size) T) as (ki, vi) eqn: HHi; Intros.
+            rewrite <- !sepcon_assoc, (sepcon_comm _ (ghost_master1 _ _)).
             rewrite (sepcon_comm _ (ghost_snap _ _)), <- !sepcon_assoc.
-            rewrite snap_master_join1, !sepcon_andp_prop'; apply view_shift_prop; intro Hk1.
-            rewrite <- (prop_true_andp _ (ghost_master _ _) Hk1).
-            rewrite <- (@snap_master_join1 _ _ _ zero_order).
-            destruct Hk1; [contradiction | subst].
-            apply derives_view_shift.
-            Exists HT.
+            rewrite snap_master_join1; Intros.
+            rewrite <- (prop_true_andp _ (ghost_master1 _ _) H28).
+            rewrite <- (@snap_master_join1 _ _ zero_order).
+            destruct H28; [contradiction | subst].
+            rewrite prop_true_andp by auto.
+            eapply derives_trans, fupd_frame_r; cancel.
+            eapply derives_trans, apply_fview_shift.
+            rewrite sepcon_comm; apply sepcon_derives; [apply derives_refl|].
             unfold hashtable; Exists T.
             rewrite extract_nth_sepcon with (i := i1 mod size)(l := map _ _)
               by (rewrite Zlength_map, Zlength_upto, Z2Nat.id; omega).
             erewrite Znth_map, Znth_upto by (rewrite ?Zlength_upto, Z2Nat.id; omega).
             unfold hashtable_entry.
-            rewrite Hpi, HHi; entailer!. }
+            rewrite Hpi, HHi; entailer!.
+            apply derives_refl. }
         Intros k2; subst.
-        match goal with |- semax _ (PROP () (LOCALx ?Q (SEPx ?R))) _ _ =>
-          forward_if (PROP (k1 = k) (LOCALx Q (SEPx R))) end.
+        forward_if (k1 = k).
         { eapply semax_pre; [|apply semax_continue].
-          unfold POSTCONDITION, abbreviate, overridePost.
-          destruct (eq_dec EK_continue EK_normal); [discriminate|].
-          unfold loop1_ret_assert.
+          unfold POSTCONDITION, abbreviate, overridePost, loop1_ret_assert, frame_ret_assert,
+            function_body_ret_assert, RA_continue.
           Exists i (i1 mod size) (upd_Znth (i1 mod size) keys k1).
           rewrite Zmod_mod, Z2Nat.inj_add, upto_app, map_app, sepcon_app by omega.
           change (upto (Z.to_nat 1)) with [0]; simpl fold_right; rewrite Z2Nat.id, Z.add_0_r by omega.
           replace ((i + hash k) mod size) with (i1 mod size); rewrite upd_Znth_same by omega; entailer!.
-          erewrite map_ext_in; eauto; simpl; intros.
+          { assert (Int.min_signed <= i1 mod size < Int.max_signed).
+            { split; etransitivity; try apply Z_mod_lt; auto; try computable.
+              setoid_rewrite (proj2_sig has_size); computable. }
+            rewrite Int.signed_repr by omega; auto. }
+          erewrite map_ext_in; [apply derives_refl|]; simpl; intros.
           rewrite upd_Znth_diff'; auto; try omega.
           replace (i1 mod size) with ((i + hash k) mod size); intro X; apply Zmod_plus_inv in X; auto.
           rewrite In_upto, Z2Nat.id in * by omega.
           rewrite !Zmod_small in X; omega. }
         { forward.
           entailer!. }
-        intros.
-        unfold exit_tycon, overridePost.
-        destruct (eq_dec ek EK_normal); [subst | apply drop_tc_environ].
-        Intros; unfold POSTCONDITION, abbreviate, normal_ret_assert, loop1_ret_assert, overridePost.
-        rewrite eq_dec_refl; entailer!.
+        entailer!.
       * forward.
         if_tac; [|contradiction].
         subst; entailer!.
-      * intros.
-        unfold exit_tycon, overridePost.
-        destruct (eq_dec ek EK_normal); [subst | apply drop_tc_environ].
-        Intros; unfold POSTCONDITION, abbreviate, normal_ret_assert, loop1_ret_assert, overridePost.
-        rewrite eq_dec_refl; entailer!.
+      * entailer!.
     + forward.
       subst; entailer!.
-    + forward; rewrite Hpi.
+    + forward; setoid_rewrite Hpi.
       { entailer!. }
-      forward_call (pvi, v, P * ghost_snap k (Znth (i1 mod size) lg Vundef) *
-          fold_right sepcon emp (map (fun i => ghost_snap (Znth ((i + hash k) mod size) keys 0)
-             (Znth ((i + hash k) mod size) lg Vundef)) (upto (Z.to_nat i))),
-        II, lI, fun sh => !!(sh = Tsh) && EX H : _, EX T : _, !!(Zlength T = size /\ wf_table T /\
-            forall k v, H k = Some v <-> In (k, v) T /\ v <> 0) && let '(ki, vi) := Znth (i1 mod size) T (0, 0) in
-        !!(ki = k /\ repable_signed vi) && ghost_master k (Znth (i1 mod size) lg Vundef) *
-        data_at Tsh tint (vint k) pki * ghost (Some H) g * fold_right sepcon emp (upd_Znth (i1 mod size)
+      forward_call (pvi, v, |> P * (AS && emp) * ghost_snap k (Znth (i1 mod size) lg) *
+          data_at sh (tarray tentry size) entries (gv _m_entries) *
+          fold_right sepcon emp (map (fun i => ghost_snap (Znth ((i + hash k) mod size) keys)
+             (Znth ((i + hash k) mod size) lg)) (upto (Z.to_nat i))),
+        Full_set iname, Empty_set iname,
+        fun sh1 => !!(sh1 = Tsh) && data_at sh (tarray tentry size) entries (gv _m_entries) *
+        EX H : _, EX T : _, !!(Zlength T = size /\ wf_table T /\
+            forall k v, H k = Some v <-> In (k, v) T /\ v <> 0) && let '(ki, vi) := Znth (i1 mod size) T in
+        !!(ki = k /\ repable_signed vi) && ghost_master1 k (Znth (i1 mod size) lg) *
+        data_at Tsh tint (vint k) pki * excl g H * fold_right sepcon emp (upd_Znth (i1 mod size)
             (map (hashtable_entry T lg entries) (upto (Z.to_nat size))) emp) *
-          R H * ghost_snap k (Znth (i1 mod size) lg Vundef) *
-          fold_right sepcon emp (map (fun i => ghost_snap (Znth ((i + hash k) mod size) keys 0)
-             (Znth ((i + hash k) mod size) lg Vundef)) (upto (Z.to_nat i))),
-       EX H' : _, Q H' tt).
-      { split; auto; split.
-        + rewrite <- !sepcon_assoc, sepcon_assoc; etransitivity; [apply view_shift_sepcon1, HP|].
-          view_shift_intro HT.
-          unfold hashtable.
-          view_shift_intro T.
+          ghost_snap k (Znth (i1 mod size) lg) *
+          fold_right sepcon emp (map (fun i => ghost_snap (Znth ((i + hash k) mod size) keys)
+             (Znth ((i + hash k) mod size) lg)) (upto (Z.to_nat i))) *
+          (ALL y : unit ,
+           weak_fview_shift (Empty_set iname) (Full_set iname)
+             (data_at sh (tarray tentry size) entries (gv _m_entries) *
+              hashtable (map_upd H k v) g lg entries) (Q y) && emp),
+        Q tt).
+      { cancel.
+        rewrite <- emp_sepcon, <- sepcon_emp at 1.
+        apply sepcon_derives; [|cancel].
+        apply sepcon_derives, derives_refl.
+        rewrite <- emp_sepcon at 1; apply sepcon_derives.
+        + unfold weak_fview_shift; rewrite <- wand_sepcon_adjoint, emp_sepcon.
+          rewrite (sepcon_comm _ (AS && emp)); unfold AS.
+          rewrite 2sepcon_assoc.
+          eapply derives_trans; [apply sepcon_derives, derives_refl; apply apply_fview_shift|].
+          eapply derives_trans; [apply fupd_frame_r | apply fupd_mono].
+          Intros HT.
+          unfold hashtable at 1; Intros T.
           rewrite extract_nth_sepcon with (i := i1 mod size)
             by (rewrite Zlength_map, Zlength_upto, Z2Nat.id; omega).
           erewrite Znth_map, Znth_upto by (rewrite ?Zlength_upto, Z2Nat.id; omega).
           unfold hashtable_entry.
           rewrite Hpi.
-          destruct (Znth (i1 mod size) T (0, 0)) as (ki, vi) eqn: HHi.
-          view_shift_intros.
-          rewrite <- !sepcon_assoc, (sepcon_comm _ (ghost_master _ _)).
+          destruct (Znth (i1 mod size) T) as (ki, vi) eqn: HHi; Intros.
+          rewrite <- !sepcon_assoc, (sepcon_comm _ (ghost_master1 _ _)).
           rewrite (sepcon_comm _ (ghost_snap _ _)), <- !sepcon_assoc.
-          rewrite snap_master_join1, !sepcon_andp_prop'; apply view_shift_prop; intro Hk1.
-          rewrite <- (prop_true_andp _ (ghost_master _ _) Hk1).
-          rewrite <- (@snap_master_join1 _ _ _ zero_order).
-          destruct Hk1; [contradiction | subst].
-          apply derives_view_shift.
+          rewrite snap_master_join1, !sepcon_andp_prop'; Intros.
+          rewrite <- (prop_true_andp _ (ghost_master1 _ _) H20).
+          rewrite <- (@snap_master_join1 _ _ zero_order).
+          destruct H20; [contradiction | subst].
+            rewrite (sepcon_comm _ (_ && _)), !sepcon_assoc.
+            eapply derives_trans; [apply sepcon_derives; [apply andp_left2|]; apply derives_refl|].
           Exists Tsh HT T; rewrite HHi; entailer!.
-        + intros.
-          view_shift_intro HT; view_shift_intro T.
-          etransitivity; [|etransitivity; [apply view_shift_sepcon with (Q' :=
-            ghost_snap k (Znth (i1 mod size) lg Vundef) *
-                      fold_right sepcon emp (map (fun i => ghost_snap (Znth ((i + hash k) mod size) keys 0)
-             (Znth ((i + hash k) mod size) lg Vundef)) (upto (Z.to_nat i))));
-            [apply (HQ HT tt) | reflexivity] | apply derives_view_shift; Exists HT; entailer!]].
-          destruct (Znth (i1 mod size) T (0, 0)) eqn: HHi.
-          view_shift_intros.
-          rewrite <- !sepcon_assoc, (sepcon_comm _(ghost (Some HT) g)), !sepcon_assoc.
-          etransitivity; [apply view_shift_sepcon1|].
+          rewrite sepcon_comm; apply derives_refl.
+        + apply allp_right; intro sh0.
+          unfold weak_fview_shift; rewrite <- wand_sepcon_adjoint, emp_sepcon.
+          Intros HT T.
+          destruct (Znth (i1 mod size) T) eqn: HHi; Intros.
+          rewrite <- !sepcon_assoc, sepcon_comm.
+          eapply derives_trans, apply_fview_shift', derives_refl.
+          apply sepcon_derives; [eapply allp_left, derives_refl|].
+          rewrite (sepcon_comm _(excl g HT)), !sepcon_assoc.
+          eapply derives_trans; [apply sepcon_derives, derives_refl|].
           { apply exclusive_update with (v' := map_upd HT k v). }
-          apply derives_view_shift.
+          eapply derives_trans; [apply bupd_frame_r|].
+          eapply derives_trans, bupd_trans; apply bupd_mono.
+          rewrite <- !sepcon_assoc, sepcon_assoc.
+          eapply derives_trans; [apply sepcon_derives; [apply derives_refl|]|].
+          { eapply derives_trans, bupd_sepcon.
+            apply sepcon_derives; [apply own_dealloc|].
+            apply snaps_dealloc. }
+          eapply derives_trans; [apply bupd_frame_l | apply bupd_mono].
           unfold hashtable.
           Exists (upd_Znth (i1 mod size) T (k, v)).
           rewrite extract_nth_sepcon with (i := i1 mod size)(l := map _ (upto (Z.to_nat size)))
@@ -713,7 +798,7 @@ Proof.
             intros; unfold map_upd; if_tac.
             * split; [intro X; inv X; split; auto; apply upd_Znth_In|].
               subst; intros (Hin & ?).
-              apply In_Znth with (d := (0, 0)) in Hin; destruct Hin as (j & Hj & Hjth).
+              apply In_Znth in Hin; destruct Hin as (j & Hj & Hjth).
               destruct (eq_dec j (i1 mod size)).
               { subst; rewrite upd_Znth_same in Hjth by omega; inv Hjth; auto. }
               rewrite upd_Znth_diff' in Hjth by (auto; omega).
@@ -724,20 +809,20 @@ Proof.
               -- eapply In_upd_Znth_old; auto; try omega.
                  rewrite HHi; intro X; inv X; contradiction.
               -- apply In_upd_Znth in Hin; destruct Hin as [X|]; [inv X; tauto | auto]. }
+          apply sepcon_derives; [apply derives_refl|].
           apply sepcon_list_derives; rewrite !upd_Znth_Zlength;
             rewrite !Zlength_map, !Zlength_upto, !Z2Nat.id; auto; try omega.
           intros; destruct (eq_dec i0 (i1 mod size)).
           { subst; rewrite !upd_Znth_same by (rewrite Zlength_map, Zlength_upto, Z2Nat.id; auto; omega); auto. }
           rewrite !upd_Znth_diff' by (rewrite ?Zlength_map, ?Zlength_upto, ?Z2Nat.id; auto; omega).
           erewrite !Znth_map, !Znth_upto by (rewrite ?Zlength_upto, Z2Nat.id; auto; omega).
-          rewrite upd_Znth_diff'; auto; omega.
-          admit. (* drop snaps *) }
-      Intros H'.
+          rewrite upd_Znth_diff'; auto; omega. }
       forward.
-      Exists tt H'; entailer!.
+      Exists tt; entailer!.
   - Intros i i1 keys.
     forward.
-    unfold loop2_ret_assert.
+    { entailer!.
+      rewrite (Int.signed_repr 1) by computable; omega. }
     Exists (i + 1) (i1 + 1) keys; entailer!.
     split.
     { rewrite <- Zplus_mod_idemp_l.
@@ -749,215 +834,266 @@ Admitted.
 Lemma body_get_item : semax_body Vprog Gprog f_get_item get_item_spec.
 Proof.
   start_atomic_function.
-  destruct x as (((((k, p), sh), entries), g), lg); Intros.
-  destruct H as (HP & HQ).
+  destruct x as (((((k, gv), sh), entries), g), lg); Intros.
   forward_call k.
   pose proof size_pos.
-  eapply semax_pre with (P' := EX i : Z, EX i1 : Z, EX keys : list Z,
+  unfold atomic_shift; Intros P.
+  set (AS := weak_fview_shift _ _ _ _).
+  forward_loop (EX i : Z, EX i1 : Z, EX keys : list Z,
     PROP (i1 mod size = (i + hash k) mod size; 0 <= i < size; Zlength keys = size;
           Forall (fun z => z <> 0 /\ z <> k) (sublist 0 i (rebase keys (hash k))))
-    LOCAL (temp _idx (vint i1); temp _key (vint k); gvar _m_entries p)
-    SEP (@data_at CompSpecs sh (tarray tentry size) entries p;
-         fold_right sepcon emp (map (fun i => ghost_snap (Znth ((i + hash k) mod size) keys 0)
-           (Znth ((i + hash k) mod size) lg Vundef)) (upto (Z.to_nat i)));
-         fold_right sepcon emp (map (fun p0 => invariant (II p0)) lI); P)).
+    LOCAL (temp _idx (vint i1); temp _key (vint k); gvars gv)
+    SEP (|> P; AS && emp; @data_at CompSpecs sh (tarray tentry size) entries (gv _m_entries);
+         fold_right sepcon emp (map (fun i => ghost_snap (Znth ((i + hash k) mod size) keys)
+           (Znth ((i + hash k) mod size) lg)) (upto (Z.to_nat i)))))%assert
+    continue: (EX i : Z, EX i1 : Z, EX keys : list Z,
+    PROP (Int.min_signed <= Int.signed (Int.repr i1) < Int.max_signed;
+          i1 mod size = (i + hash k) mod size; 0 <= i < size; Zlength keys = size;
+          Forall (fun z => z <> 0 /\ z <> k) (sublist 0 (i + 1) (rebase keys (hash k))))
+    LOCAL (temp _idx (vint i1); temp _key (vint k); gvars gv)
+    SEP (|> P; AS && emp; @data_at CompSpecs sh (tarray tentry size) entries (gv _m_entries);
+         fold_right sepcon emp (map (fun i => ghost_snap (Znth ((i + hash k) mod size) keys)
+           (Znth ((i + hash k) mod size) lg)) (upto (Z.to_nat (i + 1))))))%assert.
   { Exists 0 (k * 654435761)%Z (repeat 0 (Z.to_nat size)); rewrite sublist_nil; entailer!.
     split; [apply hash_size|].
-    rewrite Zlength_repeat, Z2Nat.id; auto; omega. }
-  eapply semax_loop.
+    rewrite Zlength_repeat, Z2Nat.id; auto; omega.
+    { simpl; auto. } }
   - Intros i i1 keys; forward.
-    forward.
     rewrite sub_repr, and_repr; simpl.
     rewrite Zland_two_p with (n := 14) by omega.
     replace (2 ^ 14) with size by (setoid_rewrite (proj2_sig has_size); auto).
     exploit (Z_mod_lt i1 size); [omega | intro Hi1].
     assert_PROP (Zlength entries = size) as Hentries by entailer!.
     assert (0 <= i1 mod size < Zlength entries) as Hi1' by omega.
-    match goal with H : Forall _ _ |- _ => pose proof (Forall_Znth _ _ _ (Vundef, Vundef) Hi1' H) as Hptr end.
-    destruct (Znth (i1 mod size) entries (Vundef, Vundef)) as (pki, pvi) eqn: Hpi; destruct Hptr.
-    forward; rewrite Hpi.
+    match goal with H : Forall _ _ |- _ => pose proof (Forall_Znth _ _ _ Hi1' H) as Hptr end.
+    destruct (Znth (i1 mod size) entries) as (pki, pvi) eqn: Hpi; destruct Hptr.
+    forward; setoid_rewrite Hpi.
     { entailer!. }
     assert (Zlength (rebase keys (hash k)) = size) as Hrebase.
     { rewrite Zlength_rebase; replace (Zlength keys) with size; auto; apply hash_range. }
-    forward_call (pki, P * fold_right sepcon emp (map (fun i0 : Z =>
-        ghost_snap (Znth ((i0 + hash k) mod size) keys 0) (Znth ((i0 + hash k) mod size) lg Vundef))
-        (upto (Z.to_nat i))), II, lI,
-      fun sh v => !!(sh = Tsh) && EX H : _, EX T : _, !!(Zlength T = size /\ wf_table T /\
-      forall k v, H k = Some v <-> In (k, v) T /\ v <> 0) && let '(ki, vi) := Znth (i1 mod size) T (0, 0) in
-      !!(v = ki /\ repable_signed vi /\ (ki = 0 -> vi = 0)) && ghost_master ki (Znth (i1 mod size) lg Vundef) *
-      data_at Tsh tint (vint vi) pvi * ghost (Some H) g * fold_right sepcon emp (upd_Znth (i1 mod size)
+    forward_call (pki, |> P * (AS && emp) * fold_right sepcon emp (map (fun i0 : Z =>
+        ghost_snap (Znth ((i0 + hash k) mod size) keys) (Znth ((i0 + hash k) mod size) lg))
+        (upto (Z.to_nat i))) * data_at sh (tarray tentry size) entries (gv _m_entries), Full_set iname, Empty_set iname,
+      fun sh1 v => !!(sh1 = Tsh) && EX H : _, EX T : _, !!(Zlength T = size /\ wf_table T /\
+      forall k v, H k = Some v <-> In (k, v) T /\ v <> 0) && let '(ki, vi) := Znth (i1 mod size) T in
+      !!(v = ki /\ repable_signed vi /\ (ki = 0 -> vi = 0)) && ghost_master1 ki (Znth (i1 mod size) lg) *
+      data_at Tsh tint (vint vi) pvi * excl g H * fold_right sepcon emp (upd_Znth (i1 mod size)
           (map (hashtable_entry T lg entries) (upto (Z.to_nat size))) emp) *
-        R H * fold_right sepcon emp (map (fun i0 : Z => ghost_snap (Znth ((i0 + hash k) mod size) keys 0)
-          (Znth ((i0 + hash k) mod size) lg Vundef)) (upto (Z.to_nat i))),
-      fun v => if eq_dec v 0 then EX H : _, Q H v else P * ghost_snap v (Znth (i1 mod size) lg Vundef) *
-        fold_right sepcon emp (map (fun i0 : Z => ghost_snap (Znth ((i0 + hash k) mod size) keys 0)
-          (Znth ((i0 + hash k) mod size) lg Vundef)) (upto (Z.to_nat i)))).
-    { split.
-      + rewrite <- !sepcon_assoc; etransitivity; [apply view_shift_sepcon1, HP|].
-        view_shift_intro HT.
-        apply derives_view_shift.
-        unfold hashtable; Intros T.
+        fold_right sepcon emp (map (fun i0 : Z => ghost_snap (Znth ((i0 + hash k) mod size) keys)
+          (Znth ((i0 + hash k) mod size) lg)) (upto (Z.to_nat i))) *
+        data_at sh (tarray tentry size) entries (gv _m_entries) *
+      (weak_fview_shift (Empty_set iname) (Full_set iname) (hashtable H g lg entries) (|> P) && emp &&
+         (ALL y : Z, weak_fview_shift (Empty_set iname) (Full_set iname)
+             (data_at sh (tarray tentry size) entries (gv _m_entries) *
+              (!! (if eq_dec y 0 then H k = None else H k = Some y) && hashtable H g lg entries))
+             (Q y) && emp)),
+      fun v => if eq_dec v 0 then Q v else |> P * ghost_snap v (Znth (i1 mod size) lg) *
+        fold_right sepcon emp (map (fun i0 : Z => ghost_snap (Znth ((i0 + hash k) mod size) keys)
+          (Znth ((i0 + hash k) mod size) lg)) (upto (Z.to_nat i))) *
+        data_at sh (tarray tentry size) entries (gv _m_entries)).
+    { rewrite emp_dup at 1; cancel.
+      rewrite sepcon_comm, <- emp_sepcon at 1.
+      rewrite <- sepcon_assoc; apply sepcon_derives; [|cancel].
+      apply sepcon_derives, derives_refl.
+      rewrite <- emp_sepcon at 1; apply sepcon_derives.
+      + unfold weak_fview_shift; rewrite <- wand_sepcon_adjoint, emp_sepcon.
+        unfold AS.
+        rewrite (sepcon_comm _ (_ && _)), sepcon_assoc.
+        eapply derives_trans; [apply sepcon_derives, derives_refl; apply apply_fview_shift|].
+        eapply derives_trans; [apply fupd_frame_r | apply fupd_mono].
+        Intros HT.
+        unfold hashtable at 1; Intros T.
         rewrite extract_nth_sepcon with (i := i1 mod size)
           by (rewrite Zlength_map, Zlength_upto, Z2Nat.id; omega).
         erewrite Znth_map, Znth_upto by (rewrite ?Zlength_upto, Z2Nat.id; omega).
         unfold hashtable_entry.
         rewrite Hpi.
-        destruct (Znth (i1 mod size) T (0, 0)) as (ki, vi) eqn: HHi.
+        destruct (Znth (i1 mod size) T) as (ki, vi) eqn: HHi.
         Intros; Exists Tsh ki HT T; rewrite HHi; entailer!.
-      + intros.
-        view_shift_intro HT; view_shift_intro T.
+        apply derives_refl.
+      + apply allp_right; intro sh0.
+        apply allp_right; intro v0.
+        unfold weak_fview_shift; rewrite <- wand_sepcon_adjoint, emp_sepcon.
+        Intros HT T.
+        destruct (Znth (i1 mod size) T) as (ki, vi) eqn: HHi; Intros.
         if_tac.
-        * etransitivity; [|etransitivity; [apply HQ | apply derives_view_shift; Exists HT; entailer!]].
-          subst; rewrite eq_dec_refl.
-          apply derives_view_shift.
+        * rewrite <- !sepcon_assoc, sepcon_comm.
+          eapply derives_trans, apply_fview_shift'.
+          { apply sepcon_derives, derives_refl.
+            eapply andp_left2, allp_left, derives_refl. }
+          subst v0 ki.
+          rewrite sepcon_comm, <- !sepcon_assoc.
+          assert_PROP (lookup T k = Some (i1 mod size)) as Hindex.
+          { rewrite sepcon_assoc, sepcon_comm.
+            apply sepcon_derives_prop, (entries_lookup k); auto.
+            rewrite HHi; auto. }
+          eapply derives_trans.
+          { apply sepcon_derives; [apply derives_refl | apply snaps_dealloc]. }
+          eapply derives_trans; [apply bupd_frame_l | apply bupd_mono].
           unfold hashtable; Exists T.
           rewrite extract_nth_sepcon with (i := i1 mod size)(l := map _ (upto (Z.to_nat size)))
             by (rewrite Zlength_map, Zlength_upto, Z2Nat.id; omega).
           erewrite Znth_map, Znth_upto by (rewrite ?Zlength_upto, Z2Nat.id; omega).
-          destruct (Znth (i1 mod size) T (0, 0)) as (ki, vi) eqn: HHi; Intros.
-          assert_PROP (lookup T k = Some (i1 mod size)) as Hindex.
-          { pose proof (entries_lookup k i i1 keys lg T entries) as Hlookup.
-            subst; sep_apply Hlookup; rewrite ?HHi; auto.
-            apply sepcon_derives_prop; auto. }
           unfold hashtable_entry.
-          rewrite Hpi, HHi; entailer!.
+          rewrite Hpi, HHi, if_true by auto; entailer!.
           destruct (HT k) eqn: Hk; auto.
           match goal with H : forall k v, _ <-> _ |- _ => rewrite H in Hk end.
-          destruct Hk as (Hk & ?); apply In_Znth with (d := (0, 0)) in Hk.
+          destruct Hk as (Hk & ?); apply In_Znth in Hk.
           destruct Hk as (j & ? & Hjth).
           match goal with H : wf_table T |- _ => exploit (H k j); rewrite ?Hjth; auto end.
           rewrite Hindex; congruence.
-          { admit. (* drop snaps *) }
-        * rewrite <- !sepcon_assoc, sepcon_assoc; etransitivity; [|apply view_shift_sepcon1, HP].
-          destruct (Znth (i1 mod size) T (0, 0)) as (ki, vi) eqn: HHi; view_shift_intros.
-          rewrite sepcon_comm.
-          rewrite !sepcon_assoc; etransitivity; [apply view_shift_sepcon1, make_snap|].
-          apply derives_view_shift; Exists HT.
+          { apply derives_refl. }
+        * rewrite sepcon_comm, !sepcon_assoc.
+          eapply derives_trans; [apply sepcon_derives, derives_refl; apply (make_snap(ORD := zero_order))|].
+          eapply derives_trans; [apply bupd_frame_r|].
+          apply fupd_bupd, bupd_mono.
+          rewrite !sepcon_assoc; eapply derives_trans, fupd_frame_r.
+          subst v0; cancel.
+          rewrite (sepcon_comm _ (_ && _)), !sepcon_assoc.
+          eapply derives_trans, apply_fview_shift'.
+          { apply sepcon_derives, derives_refl; apply andp_left1, derives_refl. }
+          eapply derives_trans, bupd_intro.
           unfold hashtable; Exists T.
           rewrite extract_nth_sepcon with (i := i1 mod size)(l := map _ (upto (Z.to_nat size)))
             by (rewrite Zlength_map, Zlength_upto, Z2Nat.id; omega).
           erewrite Znth_map, Znth_upto by (rewrite ?Zlength_upto, Z2Nat.id; omega).
           unfold hashtable_entry.
-          rewrite Hpi, HHi; entailer!. }
+          rewrite Hpi, HHi; entailer!.
+          apply derives_refl. }
     Intros k1.
-    match goal with |- semax _ (PROP () (LOCALx ?Q (SEPx ?R))) _ _ =>
-      forward_if (PROP (k1 <> k) (LOCALx Q (SEPx R))) end.
+    forward_if (k1 <> k).
     + subst; if_tac; [contradiction | Intros].
-      forward; rewrite Hpi.
+      forward; setoid_rewrite Hpi.
       { entailer!. }
-      forward_call (pvi, P * ghost_snap k (Znth (i1 mod size) lg Vundef) * fold_right sepcon emp (map (fun i0 : Z =>
-          ghost_snap (Znth ((i0 + hash k) mod size) keys 0) (Znth ((i0 + hash k) mod size) lg Vundef))
-          (upto (Z.to_nat i))), II, lI,
-        fun sh v => !!(sh = Tsh) && EX H : _, EX T : _, !!(Zlength T = size /\ wf_table T /\
-            forall k v, H k = Some v <-> In (k, v) T /\ v <> 0) && let '(ki, vi) := Znth (i1 mod size) T (0, 0) in
-        !!(ki = k /\ vi = v /\ repable_signed vi) && ghost_master k (Znth (i1 mod size) lg Vundef) *
-        data_at Tsh tint (vint k) pki * ghost (Some H) g * fold_right sepcon emp (upd_Znth (i1 mod size)
+      forward_call (pvi, |> P * (AS && emp) * ghost_snap k (Znth (i1 mod size) lg) *
+          fold_right sepcon emp (map (fun i0 : Z => ghost_snap (Znth ((i0 + hash k) mod size) keys) (Znth ((i0 + hash k) mod size) lg))
+          (upto (Z.to_nat i))) * data_at sh (tarray tentry size) entries (gv _m_entries),
+        Full_set iname, Empty_set iname,
+        fun sh1 v => !!(sh1 = Tsh) && EX H : _, EX T : _, !!(Zlength T = size /\ wf_table T /\
+            forall k v, H k = Some v <-> In (k, v) T /\ v <> 0) && let '(ki, vi) := Znth (i1 mod size) T in
+        !!(ki = k /\ vi = v /\ repable_signed vi) && ghost_master1 k (Znth (i1 mod size) lg) *
+        data_at Tsh tint (vint k) pki * excl g H * fold_right sepcon emp (upd_Znth (i1 mod size)
             (map (hashtable_entry T lg entries) (upto (Z.to_nat size))) emp) *
-          R H * ghost_snap k (Znth (i1 mod size) lg Vundef) * fold_right sepcon emp (map (fun i0 : Z =>
-            ghost_snap (Znth ((i0 + hash k) mod size) keys 0) (Znth ((i0 + hash k) mod size) lg Vundef))
-            (upto (Z.to_nat i))),
-        fun v => EX H' : _, Q H' v).
-      { split.
-        + rewrite <- !sepcon_assoc, sepcon_assoc; etransitivity; [apply view_shift_sepcon1, HP|].
-          view_shift_intro HT.
-          unfold hashtable.
-          view_shift_intro T.
+          ghost_snap k (Znth (i1 mod size) lg) * fold_right sepcon emp (map (fun i0 : Z =>
+            ghost_snap (Znth ((i0 + hash k) mod size) keys) (Znth ((i0 + hash k) mod size) lg))
+            (upto (Z.to_nat i))) * data_at sh (tarray tentry size) entries (gv _m_entries) *
+        (ALL y : Z ,
+           weak_fview_shift (Empty_set iname) (Full_set iname)
+             (data_at sh (tarray tentry size) entries (gv _m_entries) *
+              (!! (if eq_dec y 0 then H k = None else H k = Some y) && hashtable H g lg entries))
+             (Q y) && emp),
+        Q).
+      { cancel.
+        rewrite <- emp_sepcon at 1; apply sepcon_derives; [|cancel].
+        rewrite <- emp_sepcon at 1; apply sepcon_derives.
+        + unfold weak_fview_shift; rewrite <- wand_sepcon_adjoint, emp_sepcon.
+          unfold AS.
+          rewrite (sepcon_comm _ (_ && _)), 2sepcon_assoc.
+          eapply derives_trans; [apply sepcon_derives, derives_refl; apply apply_fview_shift|].
+          eapply derives_trans; [apply fupd_frame_r | apply fupd_mono].
+          Intros HT.
+          unfold hashtable at 1; Intros T.
           rewrite extract_nth_sepcon with (i := i1 mod size)
             by (rewrite Zlength_map, Zlength_upto, Z2Nat.id; omega).
           erewrite Znth_map, Znth_upto by (rewrite ?Zlength_upto, Z2Nat.id; omega).
           unfold hashtable_entry.
           rewrite Hpi.
-          destruct (Znth (i1 mod size) T (0, 0)) as (ki, vi) eqn: HHi.
-          view_shift_intros.
-          rewrite <- !sepcon_assoc, (sepcon_comm _ (ghost_master _ _)).
+          destruct (Znth (i1 mod size) T) as (ki, vi) eqn: HHi; Intros.
+          rewrite <- !sepcon_assoc, (sepcon_comm _ (ghost_master1 _ _)).
           rewrite (sepcon_comm _ (ghost_snap _ _)), <- !sepcon_assoc.
-          rewrite snap_master_join1, !sepcon_andp_prop'; apply view_shift_prop; intro Hk1.
-          rewrite <- (prop_true_andp _ (ghost_master _ _) Hk1).
-          rewrite <- (@snap_master_join1 _ _ _ zero_order).
-          destruct Hk1; [contradiction | subst].
-          apply derives_view_shift.
+          rewrite snap_master_join1, !sepcon_andp_prop'; Intros.
+          rewrite <- (prop_true_andp _ (ghost_master1 _ _) H19).
+          rewrite <- (@snap_master_join1 _ _ zero_order).
+          destruct H19; [contradiction | subst].
+          rewrite (sepcon_comm _ (_ && _)), !sepcon_assoc.
+          eapply derives_trans; [apply sepcon_derives, derives_refl; apply andp_left2, derives_refl|].
           Exists Tsh vi HT T; rewrite HHi; entailer!.
-        + intros.
-          view_shift_intro HT; view_shift_intro T.
-          destruct (Znth (i1 mod size) T (0, 0)) eqn: HHi.
-          view_shift_intros.
-          etransitivity; [|etransitivity; [apply HQ | apply derives_view_shift; Exists HT; entailer!]].
-          apply derives_view_shift.
+          rewrite sepcon_comm; apply derives_refl.
+        + apply allp_right; intro sh0.
+          apply allp_right; intro v0.
+          unfold weak_fview_shift; rewrite <- wand_sepcon_adjoint, emp_sepcon.
+          Intros HT T.
+          destruct (Znth (i1 mod size) T) eqn: HHi; Intros.
+          rewrite <- !sepcon_assoc, sepcon_comm.
+          eapply derives_trans, apply_fview_shift'.
+          { apply sepcon_derives, derives_refl.
+            eapply allp_left, derives_refl. }
+          subst; assert_PROP (lookup T k = Some (i1 mod size)) as Hindex.
+          { rewrite (sepcon_comm _ (fold_right _ _ _)), <- !sepcon_assoc,
+              (sepcon_comm _ (fold_right _ _ _)), <- !sepcon_assoc, 5sepcon_assoc.
+            apply sepcon_derives_prop, entries_lookup; auto.
+            rewrite HHi; auto. }
+          rewrite sepcon_comm, <- !sepcon_assoc, sepcon_assoc.
+          eapply derives_trans.
+          { apply sepcon_derives; [apply derives_refl|].
+            eapply derives_trans, bupd_sepcon.
+            apply sepcon_derives; [apply own_dealloc | apply snaps_dealloc]. }
+          eapply derives_trans; [apply bupd_frame_l | apply bupd_mono].
           unfold hashtable; Exists T.
           rewrite extract_nth_sepcon with (i := i1 mod size)(l := map _ (upto (Z.to_nat size)))
             by (rewrite Zlength_map, Zlength_upto, Z2Nat.id; omega).
           erewrite Znth_map, Znth_upto by (rewrite ?Zlength_upto, Z2Nat.id; omega).
-          assert_PROP (lookup T k = Some (i1 mod size)) as Hindex.
-          { pose proof (entries_lookup k i i1 keys lg T entries) as Hlookup.
-            subst; sep_apply Hlookup; rewrite ?HHi; auto.
-            apply sepcon_derives_prop; auto. }
           unfold hashtable_entry.
           rewrite Hpi, HHi; entailer!.
           if_tac.
           * destruct (HT k) eqn: Hk; auto.
             match goal with H : forall k v, _ <-> _ |- _ => rewrite H in Hk end.
-            destruct Hk as (Hk & ?); apply In_Znth with (d := (0, 0)) in Hk.
+            destruct Hk as (Hk & ?); apply In_Znth in Hk.
             destruct Hk as (j & ? & Hjth).
             match goal with H : wf_table T |- _ => exploit (H k j); rewrite ?Hjth; auto end.
             rewrite Hindex; congruence.
           * match goal with H : forall k v, ?P <-> _ |- _ => rewrite H end.
             split; auto.
-            exploit (Znth_In (i1 mod size) T (0, 0)); [omega|].
+            exploit (Znth_In (i1 mod size) T); [omega|].
             rewrite HHi; auto.
-          * admit. }
+          * apply derives_refl. }
       unfold POSTCONDITION, abbreviate; simpl map.
-      Intros v' H'; forward.
-      Exists v' H'; entailer!.
+      Intros v'; forward.
+      Exists v'; entailer!.
     + forward.
       entailer!.
-    + Intros; match goal with |- semax _ (PROP () (LOCALx ?Q (SEPx ?R))) _ _ =>
-        forward_if (PROP (k1 <> 0) (LOCALx Q (SEPx R))) end.
+    + Intros; forward_if (k1 <> 0).
       * subst; rewrite eq_dec_refl.
         unfold POSTCONDITION, abbreviate; simpl map.
-        Intro H'; forward.
-        Exists 0 H'; entailer!.
+        forward.
+        Exists 0; entailer!.
+        apply andp_left2; auto.
       * if_tac; [contradiction|].
         forward.
         entailer!.
       * intros.
-        unfold POSTCONDITION, abbreviate, overridePost.
-        if_tac; [subst | apply drop_tc_environ].
-        unfold loop1_ret_assert.
-        instantiate (1 := EX i : Z, EX i1 : Z, EX keys : list Z,
-          PROP (i1 mod size = (i + hash k) mod size; 0 <= i < size; Zlength keys = size;
-            Forall (fun z => z <> 0 /\ z <> k) (sublist 0 (i + 1) (rebase keys (hash k))))
-          LOCAL (temp _idx (vint i1); temp _key (vint k); gvar _m_entries p)
-          SEP (@data_at CompSpecs sh (tarray tentry size) entries p;
-               fold_right sepcon emp (map (fun i0 : Z =>
-                 ghost_snap (Znth ((i0 + hash k) mod size) keys 0) (Znth ((i0 + hash k) mod size) lg Vundef))
-                 (upto (Z.to_nat (i + 1))));
-               fold_right sepcon emp (map (fun p0 => invariant (II p0)) lI); P)).
-        Intros; Exists i (i1 mod size) (upd_Znth (i1 mod size) keys k1).
+        Exists i (i1 mod size) (upd_Znth (i1 mod size) keys k1).
         rewrite Z2Nat.inj_add, upto_app, map_app, sepcon_app by omega.
         change (upto (Z.to_nat 1)) with [0]; simpl fold_right.
         rewrite Z2Nat.id, Z.add_0_r by omega.
-        if_tac; [contradiction|].
+        Intros; rewrite if_false by auto.
         replace ((i + hash k) mod size) with (i1 mod size); rewrite upd_Znth_same by omega; entailer!.
-        { split; [rewrite Zmod_mod; auto|].
+        { split.
+          { assert (Int.min_signed <= i1 mod size < Int.max_signed).
+            { split; etransitivity; try apply Z_mod_lt; auto; try computable.
+              setoid_rewrite (proj2_sig has_size); computable. }
+            rewrite Int.signed_repr by omega; auto. }
+          split; [rewrite Zmod_mod; auto|].
           split; [rewrite upd_Znth_Zlength; auto; omega|].
           replace (i1 mod size) with ((i + hash k) mod size); replace size with (Zlength keys);
             rewrite !rebase_upd' by (try omega; replace (Zlength keys) with size; apply Z_mod_lt; omega).
           rewrite sublist_upd_Znth_lr by (try omega; setoid_rewrite Hrebase; omega).
-          rewrite sublist_split with (mid := i), sublist_len_1 with (d := 0) by (try omega; setoid_rewrite Hrebase; omega).
+          rewrite sublist_split with (mid := i), sublist_len_1 by (try omega; setoid_rewrite Hrebase; omega).
           rewrite Z.sub_0_r, upd_Znth_app2, Forall_app; rewrite Zlength_sublist;
             rewrite ?Zlength_cons, ?Zlength_nil; try omega; try (setoid_rewrite Hrebase; omega).
           split; auto.
           rewrite Z.sub_0_r, Zminus_diag, upd_Znth0, Zlength_cons, sublist_1_cons, sublist_same
             by (auto; omega).
           repeat constructor; auto; tauto. }
-        erewrite map_ext_in; eauto; intros; simpl.
+        erewrite map_ext_in; [apply derives_refl|]; intros; simpl.
         rewrite upd_Znth_diff'; auto; try omega.
         replace (i1 mod size) with ((i + hash k) mod size); intro X; apply Zmod_plus_inv in X; auto.
         rewrite In_upto, Z2Nat.id in * by omega.
         rewrite !Zmod_small in X; omega.
   - Intros i i1 keys.
     forward.
-    unfold loop2_ret_assert.
+    { entailer!.
+      rewrite (Int.signed_repr 1) by computable; omega. }
     Exists (i + 1) (i1 + 1) keys; entailer!.
     split.
     { rewrite <- Zplus_mod_idemp_l.
@@ -969,74 +1105,97 @@ Admitted.
 Lemma body_add_item : semax_body Vprog Gprog f_add_item add_item_spec.
 Proof.
   start_atomic_function.
-  destruct x as ((((((k, v), p), sh), entries), g), lg); Intros.
-  destruct H as (HP & HQ).
+  destruct x as ((((((k, v), gv), sh), entries), g), lg); Intros.
+  unfold atomic_shift; Intros P.
+  set (AS := weak_fview_shift _ _ _ _).
   forward_call k.
   pose proof size_pos.
-  eapply semax_pre with (P' := EX i : Z, EX i1 : Z, EX keys : list Z,
+  forward_loop (EX i : Z, EX i1 : Z, EX keys : list Z,
     PROP (i1 mod size = (i + hash k) mod size; 0 <= i < size; Zlength keys = size;
           Forall (fun z => z <> 0 /\ z <> k) (sublist 0 i (rebase keys (hash k))))
-    LOCAL (temp _idx (vint i1); temp _key (vint k); temp _value (vint v); gvar _m_entries p)
-    SEP (@data_at CompSpecs sh (tarray tentry size) entries p;
-         fold_right sepcon emp (map (fun i => ghost_snap (Znth ((i + hash k) mod size) keys 0)
-           (Znth ((i + hash k) mod size) lg Vundef)) (upto (Z.to_nat i)));
-         fold_right sepcon emp (map (fun p0 => invariant (II p0)) lI); P)).
+    LOCAL (temp _idx (vint i1); temp _key (vint k); temp _value (vint v); gvars gv)
+    SEP (|> P; AS && emp; @data_at CompSpecs sh (tarray tentry size) entries (gv _m_entries);
+         fold_right sepcon emp (map (fun i => ghost_snap (Znth ((i + hash k) mod size) keys)
+           (Znth ((i + hash k) mod size) lg)) (upto (Z.to_nat i)))))%assert
+    continue: (EX i : Z, EX i1 : Z, EX keys : list Z,
+    PROP (Int.min_signed <= Int.signed (Int.repr i1) < Int.max_signed;
+          i1 mod size = (i + hash k) mod size; 0 <= i < size; Zlength keys = size;
+          Forall (fun z => z <> 0 /\ z <> k) (sublist 0 (i + 1) (rebase keys (hash k))))
+    LOCAL (temp _idx (vint i1); temp _key (vint k); temp _value (vint v); gvars gv)
+    SEP (|> P; AS && emp; @data_at CompSpecs sh (tarray tentry size) entries (gv _m_entries);
+         fold_right sepcon emp (map (fun i => ghost_snap (Znth ((i + hash k) mod size) keys)
+           (Znth ((i + hash k) mod size) lg)) (upto (Z.to_nat (i + 1))))))%assert.
   { Exists 0 (k * 654435761)%Z (repeat 0 (Z.to_nat size)); rewrite sublist_nil; entailer!.
     split; [apply hash_size|].
-    rewrite Zlength_repeat, Z2Nat.id; auto; omega. }
-  eapply semax_loop.
+    rewrite Zlength_repeat, Z2Nat.id; auto; omega.
+    { simpl; auto. } }
   - Intros i i1 keys; forward.
-    forward.
     rewrite sub_repr, and_repr; simpl.
     rewrite Zland_two_p with (n := 14) by omega.
     replace (2 ^ 14) with size by (setoid_rewrite (proj2_sig has_size); auto).
     exploit (Z_mod_lt i1 size); [omega | intro Hi1].
     assert_PROP (Zlength entries = size) as Hentries by entailer!.
     assert (0 <= i1 mod size < Zlength entries) as Hi1' by omega.
-    match goal with H : Forall _ _ |- _ => pose proof (Forall_Znth _ _ _ (Vundef, Vundef) Hi1' H) as Hptr end.
-    destruct (Znth (i1 mod size) entries (Vundef, Vundef)) as (pki, pvi) eqn: Hpi; destruct Hptr.
-    forward; rewrite Hpi.
+    match goal with H : Forall _ _ |- _ => pose proof (Forall_Znth _ _ _ Hi1' H) as Hptr end.
+    destruct (Znth (i1 mod size) entries) as (pki, pvi) eqn: Hpi; destruct Hptr.
+    forward; setoid_rewrite Hpi.
     { entailer!. }
     assert (Zlength (rebase keys (hash k)) = size) as Hrebase.
     { rewrite Zlength_rebase; replace (Zlength keys) with size; auto; apply hash_range. }
-    forward_call (pki, P, II, lI,
+    forward_call (pki, |> P * (AS && emp), Full_set iname, Empty_set iname,
       fun sh v => !!(sh = Tsh) && EX H : _, EX T : _, !!(Zlength T = size /\ wf_table T /\
-      forall k v, H k = Some v <-> In (k, v) T /\ v <> 0) && let '(ki, vi) := Znth (i1 mod size) T (0, 0) in
-      !!(v = ki /\ repable_signed vi /\ (ki = 0 -> vi = 0)) && ghost_master ki (Znth (i1 mod size) lg Vundef) *
-      data_at Tsh tint (vint vi) pvi * ghost (Some H) g * fold_right sepcon emp (upd_Znth (i1 mod size)
-          (map (hashtable_entry T lg entries) (upto (Z.to_nat size))) emp) * R H,
-      fun v : Z => P * ghost_snap v (Znth (i1 mod size) lg Vundef)).
-    { split.
-      + etransitivity; [apply HP|].
-        view_shift_intro HT.
-        apply derives_view_shift.
-        unfold hashtable; Intros T.
+      forall k v, H k = Some v <-> In (k, v) T /\ v <> 0) && let '(ki, vi) := Znth (i1 mod size) T in
+      !!(v = ki /\ repable_signed vi /\ (ki = 0 -> vi = 0)) && ghost_master1 ki (Znth (i1 mod size) lg) *
+      data_at Tsh tint (vint vi) pvi * excl g H * fold_right sepcon emp (upd_Znth (i1 mod size)
+          (map (hashtable_entry T lg entries) (upto (Z.to_nat size))) emp) *
+      (weak_fview_shift (Empty_set iname) (Full_set iname) (hashtable H g lg entries) (|> P) && emp),
+      fun v : Z => |> P * ghost_snap v (Znth (i1 mod size) lg)).
+    { rewrite emp_dup at 1; cancel.
+      rewrite <- emp_sepcon at 1; apply sepcon_derives; [|cancel].
+      rewrite <- emp_sepcon at 1; apply sepcon_derives.
+      + unfold weak_fview_shift; rewrite <- wand_sepcon_adjoint, emp_sepcon.
+        unfold AS.
+        rewrite sepcon_comm.
+        eapply derives_trans; [apply apply_fview_shift|].
+        apply fupd_mono.
+        Intros HT.
+        unfold hashtable at 1; Intros T.
         rewrite extract_nth_sepcon with (i := i1 mod size)
           by (rewrite Zlength_map, Zlength_upto, Z2Nat.id; omega).
         erewrite Znth_map, Znth_upto by (rewrite ?Zlength_upto, Z2Nat.id; omega).
         unfold hashtable_entry.
         rewrite Hpi.
-        destruct (Znth (i1 mod size) T (0, 0)) as (ki, vi) eqn: HHi.
+        destruct (Znth (i1 mod size) T) as (ki, vi) eqn: HHi.
+        rewrite <- !sepcon_assoc.
+        eapply derives_trans; [apply sepcon_derives, andp_left1; apply derives_refl|].
         Intros; Exists Tsh ki HT T; rewrite HHi; entailer!.
-      + intros.
-        rewrite <- sepcon_assoc; etransitivity; [|apply view_shift_sepcon1, HP].
-        view_shift_intro HT.
-        view_shift_intro T.
-        destruct (Znth (i1 mod size) T (0, 0)) as (ki, vi) eqn: HHi; view_shift_intros.
-        rewrite <- !sepcon_assoc, (sepcon_comm _ (ghost_master _ _)).
-        rewrite !sepcon_assoc; etransitivity; [apply view_shift_sepcon1, make_snap|].
-        apply derives_view_shift.
-        Exists HT.
+        apply derives_refl.
+      + apply allp_right; intro sh0.
+        apply allp_right; intro v0.
+        unfold weak_fview_shift; rewrite <- wand_sepcon_adjoint, emp_sepcon.
+        Intros HT T.
+        destruct (Znth (i1 mod size) T) as (ki, vi) eqn: HHi; Intros.
+        rewrite <- !sepcon_assoc, (sepcon_comm _ (ghost_master1 _ _)).
+        rewrite !sepcon_assoc; eapply derives_trans.
+        { apply sepcon_derives, derives_refl.
+          apply (make_snap(ORD := zero_order)). }
+        eapply derives_trans; [apply bupd_frame_r|].
+        apply fupd_bupd, bupd_mono.
+        eapply derives_trans, fupd_frame_r.
+        subst v0; cancel.
+        rewrite sepcon_comm; apply apply_fview_shift'.
+        eapply derives_trans, bupd_intro.
         unfold hashtable; Exists T.
         rewrite extract_nth_sepcon with (i := i1 mod size)(l := map _ _)
           by (rewrite Zlength_map, Zlength_upto, Z2Nat.id; omega).
         erewrite Znth_map, Znth_upto by (rewrite ?Zlength_upto, Z2Nat.id; omega).
         unfold hashtable_entry.
-        rewrite Hpi, HHi; entailer!. }
+        rewrite Hpi, HHi; entailer!.
+        apply derives_refl. }
     Intros k1.
-    focus_SEP 2.
+    focus_SEP 1.
     match goal with |- semax _ (PROP () (LOCALx (_ :: ?Q) (SEPx (_ :: ?R)))) _ _ =>
-      forward_if (PROP () (LOCALx Q (SEPx (ghost_snap k (Znth (i1 mod size) lg Vundef) :: R)))) end.
+      forward_if (PROP () (LOCALx Q (SEPx (ghost_snap k (Znth (i1 mod size) lg) :: R)))) end.
     + assert (forall k1, (k1 <> k /\ k1 <> 0) ->
         Zlength (upd_Znth (i1 mod size) keys k1) = size /\
         Forall (fun z => z <> 0 /\ z <> k)
@@ -1045,33 +1204,27 @@ Proof.
         replace (i1 mod size) with ((i + hash k) mod size); replace size with (Zlength keys);
           rewrite !rebase_upd' by (try omega; replace (Zlength keys) with size; apply Z_mod_lt; omega).
         rewrite sublist_upd_Znth_lr by (try omega; setoid_rewrite Hrebase; omega).
-        rewrite sublist_split with (mid := i), sublist_len_1 with (d := 0) by (try omega; setoid_rewrite Hrebase; omega).
+        rewrite sublist_split with (mid := i), sublist_len_1 by (try omega; setoid_rewrite Hrebase; omega).
         rewrite Z.sub_0_r, upd_Znth_app2, Forall_app; rewrite Zlength_sublist;
           rewrite ?Zlength_cons, ?Zlength_nil; try omega; try (setoid_rewrite Hrebase; omega).
         split; auto.
         rewrite Z.sub_0_r, Zminus_diag, upd_Znth0, Zlength_cons, sublist_1_cons, sublist_same
           by (auto; omega).
         repeat constructor; auto; tauto. }
-      match goal with |- semax _ (PROP () (LOCALx ?Q (SEPx ?R))) _ _ =>
-        forward_if (PROP (k1 = 0) (LOCALx Q (SEPx R))) end.
+      forward_if (k1 = 0).
       { eapply semax_pre; [|apply semax_continue].
-        unfold POSTCONDITION, abbreviate, overridePost.
-        destruct (eq_dec EK_continue EK_normal); [discriminate|].
-        unfold loop1_ret_assert.
-        instantiate (1 := EX i : Z, EX i1 : Z, EX keys : list Z,
-          PROP (i1 mod size = (i + hash k) mod size; 0 <= i < size; Zlength keys = size;
-            Forall (fun z => z <> 0 /\ z <> k) (sublist 0 (i + 1) (rebase keys (hash k))))
-          LOCAL (temp _idx (vint i1); temp _key (vint k); temp _value (vint v); gvar _m_entries p)
-          SEP (@data_at CompSpecs sh (tarray tentry size) entries p;
-               fold_right sepcon emp (map (fun i => ghost_snap (Znth ((i + hash k) mod size) keys 0)
-                 (Znth ((i + hash k) mod size) lg Vundef)) (upto (Z.to_nat (i + 1))));
-               fold_right sepcon emp (map (fun p0 => invariant (II p0)) lI); P)).
+        unfold POSTCONDITION, abbreviate, overridePost, loop1_ret_assert, frame_ret_assert,
+          function_body_ret_assert, RA_continue.
         Exists i (i1 mod size) (upd_Znth (i1 mod size) keys k1).
         rewrite Zmod_mod, Z2Nat.inj_add, upto_app, map_app, sepcon_app by omega.
         change (upto (Z.to_nat 1)) with [0]; simpl fold_right.
         rewrite Z2Nat.id, Z.add_0_r by omega.
         replace ((i + hash k) mod size) with (i1 mod size); rewrite upd_Znth_same by omega; entailer!.
-        erewrite map_ext_in; eauto; intros; simpl.
+        { assert (Int.min_signed <= i1 mod size < Int.max_signed).
+          { split; etransitivity; try apply Z_mod_lt; auto; try computable.
+            setoid_rewrite (proj2_sig has_size); computable. }
+          rewrite Int.signed_repr by omega; auto. }
+        erewrite map_ext_in; [apply derives_refl|]; intros; simpl.
         rewrite upd_Znth_diff'; auto; try omega.
         replace (i1 mod size) with ((i + hash k) mod size); intro X; apply Zmod_plus_inv in X; auto.
         rewrite In_upto, Z2Nat.id in * by omega.
@@ -1079,55 +1232,74 @@ Proof.
       { forward.
         entailer!. }
       Intros; subst.
-      forward_call (pki, 0, k, P * ghost_snap 0 (Znth (i1 mod size) lg Vundef) *
-          fold_right sepcon emp (map (fun i => ghost_snap (Znth ((i + hash k) mod size) keys 0)
-            (Znth ((i + hash k) mod size) lg Vundef)) (upto (Z.to_nat i))),
-        II, lI, fun sh v => !!(sh = Tsh) && EX H : _, EX T : _, !!(Zlength T = size /\ wf_table T /\
-          forall k v, H k = Some v <-> In (k, v) T /\ v <> 0) && let '(ki, vi) := Znth (i1 mod size) T (0, 0) in
+      forward_call (pki, 0, k, |> P * (AS && emp) * ghost_snap 0 (Znth (i1 mod size) lg) *
+          fold_right sepcon emp (map (fun i => ghost_snap (Znth ((i + hash k) mod size) keys)
+            (Znth ((i + hash k) mod size) lg)) (upto (Z.to_nat i))),
+        Full_set iname, Empty_set iname, fun sh v => !!(sh = Tsh) && EX H : _, EX T : _,
+          !!(Zlength T = size /\ wf_table T /\
+          forall k v, H k = Some v <-> In (k, v) T /\ v <> 0) && let '(ki, vi) := Znth (i1 mod size) T in
           !!(v = ki /\ repable_signed vi /\ (ki = 0 -> vi = 0)) &&
-          ghost_master ki (Znth (i1 mod size) lg Vundef) * data_at Tsh tint (vint vi) pvi *
-          ghost (Some H) g * fold_right sepcon emp (upd_Znth (i1 mod size)
+          ghost_master1 ki (Znth (i1 mod size) lg) * data_at Tsh tint (vint vi) pvi *
+          excl g H * fold_right sepcon emp (upd_Znth (i1 mod size)
             (map (hashtable_entry T lg entries) (upto (Z.to_nat size))) emp) *
-          R H * ghost_snap 0 (Znth (i1 mod size) lg Vundef) *
-          fold_right sepcon emp (map (fun i => ghost_snap (Znth ((i + hash k) mod size) keys 0)
-           (Znth ((i + hash k) mod size) lg Vundef)) (upto (Z.to_nat i))),
-        fun v : Z => P * ghost_snap (if eq_dec v 0 then k else v) (Znth (i1 mod size) lg Vundef) *
-          fold_right sepcon emp (map (fun i => ghost_snap (Znth ((i + hash k) mod size) keys 0)
-            (Znth ((i + hash k) mod size) lg Vundef)) (upto (Z.to_nat i)))).
-      { repeat (split; auto).
-        * rewrite <- !sepcon_assoc, sepcon_assoc; etransitivity; [apply view_shift_sepcon1, HP|].
-          view_shift_intro HT.
-          apply derives_view_shift.
-          unfold hashtable; Intros T.
+          ghost_snap 0 (Znth (i1 mod size) lg) *
+          fold_right sepcon emp (map (fun i => ghost_snap (Znth ((i + hash k) mod size) keys)
+           (Znth ((i + hash k) mod size) lg)) (upto (Z.to_nat i))) *
+          (weak_fview_shift (Empty_set iname) (Full_set iname) (hashtable H g lg entries) (|> P) && emp),
+        fun v : Z => |> P * ghost_snap (if eq_dec v 0 then k else v) (Znth (i1 mod size) lg) *
+          fold_right sepcon emp (map (fun i => ghost_snap (Znth ((i + hash k) mod size) keys)
+            (Znth ((i + hash k) mod size) lg)) (upto (Z.to_nat i)))).
+      { rewrite emp_dup at 1.
+        cancel.
+        rewrite sepcon_comm, <- emp_sepcon at 1.
+        rewrite <- sepcon_assoc.
+        apply sepcon_derives; [|cancel]; apply sepcon_derives, derives_refl.
+        rewrite <- emp_sepcon at 1; apply sepcon_derives.
+        * unfold weak_fview_shift; rewrite <- wand_sepcon_adjoint, emp_sepcon.
+          rewrite sepcon_assoc, (sepcon_comm _ (AS && emp)); unfold AS.
+          eapply derives_trans; [apply sepcon_derives, derives_refl; apply apply_fview_shift|].
+          eapply derives_trans; [apply fupd_frame_r | apply fupd_mono].
+          Intros HT.
+          unfold hashtable at 1; Intros T.
           rewrite extract_nth_sepcon with (i := i1 mod size) by (rewrite Zlength_map, Zlength_upto, Z2Nat.id; omega).
           erewrite Znth_map, Znth_upto by (rewrite ?Zlength_upto, Z2Nat.id; omega).
           unfold hashtable_entry.
           rewrite Hpi.
-          destruct (Znth (i1 mod size) T (0, 0)) as (ki, vi) eqn: HHi.
-          Exists Tsh ki HT T; rewrite HHi; entailer!.
-        * intros.
-          rewrite <- !sepcon_assoc, sepcon_assoc; etransitivity; [|apply view_shift_sepcon1, HP].
-          view_shift_intro HT; view_shift_intro T.
-          destruct (Znth (i1 mod size) T (0, 0)) as (ki, vi) eqn: HHi.
-          view_shift_intros.
+          destruct (Znth (i1 mod size) T) as (ki, vi) eqn: HHi; Intros.
+          rewrite (sepcon_comm _ (_ && _)), !sepcon_assoc.
+          eapply derives_trans; [apply sepcon_derives; [apply andp_left1|]; apply derives_refl|].
+          Exists Tsh ki HT T; rewrite HHi; unfold weak_fview_shift; entailer!.
+          apply derives_refl.
+        * apply allp_right; intro sh0.
+          apply allp_right; intro v0.
+          unfold weak_fview_shift; rewrite <- wand_sepcon_adjoint, emp_sepcon.
+          Intros HT T.
+          destruct (Znth (i1 mod size) T) as (ki, vi) eqn: HHi; Intros.
           assert (0 <= i1 mod size < Zlength T) by omega.
-          rewrite <- !sepcon_assoc, (sepcon_comm _ (ghost_master _ _)).
+          rewrite <- !sepcon_assoc, (sepcon_comm _ (ghost_master1 _ _)).
           rewrite (sepcon_comm _ (ghost_snap _ _)), <- !sepcon_assoc.
-          rewrite 5sepcon_assoc; etransitivity; [apply view_shift_sepcon1|].
+          rewrite 5sepcon_assoc; eapply derives_trans; [apply sepcon_derives, derives_refl|].
           { apply snap_master_update1 with (v' := if eq_dec ki 0 then k else ki).
             if_tac; auto. }
-          apply derives_view_shift.
+          eapply derives_trans; [apply bupd_frame_r | apply fupd_bupd, bupd_mono].
           assert (0 <= hash k < Zlength T) by (replace (Zlength T) with size; apply hash_range).
           assert (0 <= i < Zlength (rebase T (hash k))) by (rewrite Zlength_rebase; auto; omega).
-          assert (fst (Znth i (rebase T (hash k)) (0, 0)) = ki).
+          assert (fst (Znth i (rebase T (hash k))) = ki).
           { rewrite Znth_rebase by (auto; omega).
             replace (Zlength T) with size; replace ((i + hash k) mod size) with (i1 mod size); rewrite HHi; auto. }
           assert_PROP ((ki = k \/ ki = 0) -> lookup T k = Some (i1 mod size)) as Hindex.
           { rewrite prop_forall; apply allp_right; intro Hki.
-            pose proof (entries_lookup k i i1 keys lg T entries) as Hlookup.
-            sep_apply Hlookup; rewrite ?HHi; auto.
-            apply sepcon_derives_prop; auto. }
-          Exists HT.
+            rewrite <- !sepcon_assoc, (sepcon_comm _ (fold_right sepcon emp _)),
+              <- !sepcon_assoc, (sepcon_comm _ (fold_right sepcon emp _)).
+            rewrite <- !sepcon_assoc, 5sepcon_assoc.
+            apply sepcon_derives_prop, entries_lookup; auto.
+            rewrite HHi; auto. }
+          rewrite !sepcon_assoc; eapply derives_trans, fupd_frame_r.
+          subst v0; cancel.
+          rewrite (sepcon_comm _ (ghost_snap _ _)), !sepcon_assoc; apply sepcon_derives; [apply derives_refl|].
+          rewrite <- !sepcon_assoc, sepcon_comm.
+          eapply derives_trans, apply_fview_shift.
+          apply sepcon_derives; [apply derives_refl|].
           unfold hashtable; Exists (upd_Znth (i1 mod size) T (if eq_dec ki 0 then k else ki, vi)).
           rewrite extract_nth_sepcon with (i := i1 mod size)(l := map _ (upto (Z.to_nat size)))
             by (rewrite Zlength_map, Zlength_upto, Z2Nat.id; omega).
@@ -1143,6 +1315,7 @@ Proof.
             - eapply In_upd_Znth_old; auto; try omega.
               rewrite HHi; intro X; inv X; tauto.
             - apply In_upd_Znth in Hin; destruct Hin as [X|]; [inv X; tauto | auto]. }
+          apply sepcon_derives; [apply derives_refl|].
           apply sepcon_list_derives; rewrite !upd_Znth_Zlength;
             rewrite !Zlength_map, !Zlength_upto, !Z2Nat.id; auto; try omega.
           intros; destruct (eq_dec i0 (i1 mod size)).
@@ -1151,135 +1324,168 @@ Proof.
           erewrite !Znth_map, !Znth_upto by (rewrite ?Zlength_upto, Z2Nat.id; auto; omega).
           rewrite upd_Znth_diff'; auto. }
       Intros k1.
-      focus_SEP 2.
+      focus_SEP 1.
       match goal with |- semax _ (PROP () (LOCALx (_ :: _ :: ?Q) (SEPx (_ :: ?R)))) _ _ =>
-        forward_if (PROP () ((LOCALx Q) (SEPx (ghost_snap k (Znth (i1 mod size) lg Vundef) :: R)))) end.
+        forward_if (PROP () ((LOCALx Q) (SEPx (ghost_snap k (Znth (i1 mod size) lg) :: R)))) end.
       * if_tac; [discriminate|].
-        forward_call (pki, P * ghost_snap k1 (Znth (i1 mod size) lg Vundef), II, lI,
+        forward_call (pki, |> P * (AS && emp) * ghost_snap k1 (Znth (i1 mod size) lg), Full_set iname, Empty_set iname,
           fun sh v => !!(sh = Tsh) && EX H : _, EX T : _, !!(Zlength T = size /\ wf_table T /\
-            forall k v, H k = Some v <-> In (k, v) T /\ v <> 0) && let '(ki, vi) := Znth (i1 mod size) T (0, 0) in
+            forall k v, H k = Some v <-> In (k, v) T /\ v <> 0) && let '(ki, vi) := Znth (i1 mod size) T in
             !!(v = ki /\ repable_signed vi /\ (ki = 0 -> vi = 0)) &&
-            ghost_master ki (Znth (i1 mod size) lg Vundef) * data_at Tsh tint (vint vi) pvi *
-            ghost (Some H) g * fold_right sepcon emp (upd_Znth (i1 mod size)
+            ghost_master1 ki (Znth (i1 mod size) lg) * data_at Tsh tint (vint vi) pvi *
+            excl g H * fold_right sepcon emp (upd_Znth (i1 mod size)
               (map (hashtable_entry T lg entries) (upto (Z.to_nat size))) emp) *
-            R H * ghost_snap k1 (Znth (i1 mod size) lg Vundef),
-          fun v : Z => P * (!!(v = k1) && ghost_snap k1 (Znth (i1 mod size) lg Vundef))).
-        { split.
-          + rewrite <- sepcon_assoc; etransitivity; [apply view_shift_sepcon; [apply HP | reflexivity]|].
-            view_shift_intro HT.
-            apply derives_view_shift.
-            unfold hashtable; Intros T.
+            ghost_snap k1 (Znth (i1 mod size) lg) *
+            (weak_fview_shift (Empty_set iname) (Full_set iname) (hashtable H g lg entries) (|> P) && emp),
+          fun v : Z => |> P * (!!(v = k1) && ghost_snap k1 (Znth (i1 mod size) lg))).
+        { rewrite emp_dup at 1.
+          cancel.
+          rewrite <- emp_sepcon at 1; apply sepcon_derives; [|cancel].
+          rewrite <- emp_sepcon at 1; apply sepcon_derives.
+          * unfold weak_fview_shift; rewrite <- wand_sepcon_adjoint, emp_sepcon.
+            rewrite (sepcon_comm _ (AS && emp)); unfold AS.
+            eapply derives_trans; [apply sepcon_derives, derives_refl; apply apply_fview_shift|].
+            eapply derives_trans; [apply fupd_frame_r | apply fupd_mono].
+            Intros HT.
+            unfold hashtable at 1; Intros T.
             rewrite extract_nth_sepcon with (i := i1 mod size)
               by (rewrite Zlength_map, Zlength_upto, Z2Nat.id; omega).
             erewrite Znth_map, Znth_upto by (rewrite ?Zlength_upto, Z2Nat.id; omega).
             unfold hashtable_entry.
             rewrite Hpi.
-            destruct (Znth (i1 mod size) T (0, 0)) as (ki, vi) eqn: HHi.
+            destruct (Znth (i1 mod size) T) as (ki, vi) eqn: HHi; Intros.
+            rewrite (sepcon_comm _ (_ && _)), !sepcon_assoc.
+            eapply derives_trans; [apply sepcon_derives; [apply andp_left1|]; apply derives_refl|].
             Exists Tsh ki HT T; rewrite HHi; entailer!.
-          + intros.
-            rewrite <- sepcon_assoc; etransitivity; [|apply view_shift_sepcon; [apply HP | reflexivity]].
-            view_shift_intro HT; view_shift_intro T.
-            destruct (Znth (i1 mod size) T (0, 0)) as (ki, vi) eqn: HHi.
-            view_shift_intros.
-            rewrite <- !sepcon_assoc, (sepcon_comm _ (ghost_master _ _)).
+            apply derives_refl.
+          * apply allp_right; intro sh0.
+            apply allp_right; intro v0.
+            unfold weak_fview_shift; rewrite <- wand_sepcon_adjoint, emp_sepcon.
+            Intros HT T.
+            destruct (Znth (i1 mod size) T) as (ki, vi) eqn: HHi; Intros.
+            rewrite <- !sepcon_assoc, (sepcon_comm _ (ghost_master1 _ _)).
             rewrite (sepcon_comm _ (ghost_snap _ _)), <- !sepcon_assoc.
-            rewrite snap_master_join1, !sepcon_andp_prop'; apply view_shift_prop; intro Hk1.
-            rewrite <- (prop_true_andp _ (ghost_master _ _) Hk1).
-            rewrite <- (@snap_master_join1 _ _ _ zero_order).
-            destruct Hk1; [contradiction | subst].
-            apply derives_view_shift.
-            Exists HT.
+            rewrite snap_master_join1, !sepcon_andp_prop'; Intros.
+            rewrite <- (prop_true_andp _ (ghost_master1 _ _) H28).
+            rewrite <- (@snap_master_join1 _ _ zero_order).
+            destruct H28; [contradiction | subst].
+            rewrite prop_true_andp by auto.
+            eapply derives_trans, fupd_frame_r; cancel.
+            rewrite sepcon_comm; apply apply_fview_shift'.
+            eapply derives_trans, bupd_intro.
             unfold hashtable; Exists T.
             rewrite extract_nth_sepcon with (i := i1 mod size)(l := map _ _)
               by (rewrite Zlength_map, Zlength_upto, Z2Nat.id; omega).
             erewrite Znth_map, Znth_upto by (rewrite ?Zlength_upto, Z2Nat.id; omega).
             unfold hashtable_entry.
-            rewrite Hpi, HHi; entailer!. }
+            rewrite Hpi, HHi; entailer!.
+            apply derives_refl. }
         Intros k2; subst.
-        match goal with |- semax _ (PROP () (LOCALx ?Q (SEPx ?R))) _ _ =>
-          forward_if (PROP (k1 = k) (LOCALx Q (SEPx R))) end.
+        forward_if (k1 = k).
         { eapply semax_pre; [|apply semax_continue].
-          unfold POSTCONDITION, abbreviate, overridePost.
-          destruct (eq_dec EK_continue EK_normal); [discriminate|].
-          unfold loop1_ret_assert.
+          unfold POSTCONDITION, abbreviate, overridePost, loop1_ret_assert, frame_ret_assert,
+            function_body_ret_assert, RA_continue.
           Exists i (i1 mod size) (upd_Znth (i1 mod size) keys k1).
           rewrite Zmod_mod, Z2Nat.inj_add, upto_app, map_app, sepcon_app by omega.
           change (upto (Z.to_nat 1)) with [0]; simpl fold_right.
           rewrite Z2Nat.id, Z.add_0_r by omega.
           replace ((i + hash k) mod size) with (i1 mod size); rewrite upd_Znth_same by omega; entailer!.
-          erewrite map_ext_in; eauto; intros; simpl.
+          { assert (Int.min_signed <= i1 mod size < Int.max_signed).
+          { split; etransitivity; try apply Z_mod_lt; auto; try computable.
+            setoid_rewrite (proj2_sig has_size); computable. }
+          rewrite Int.signed_repr by omega; auto. }
+          erewrite map_ext_in; [apply derives_refl|]; intros; simpl.
           rewrite upd_Znth_diff'; auto; try omega.
           replace (i1 mod size) with ((i + hash k) mod size); intro X; apply Zmod_plus_inv in X; auto.
           rewrite In_upto, Z2Nat.id in * by omega.
           rewrite !Zmod_small in X; omega. }
         { forward.
           entailer!. }
-        intros.
-        unfold exit_tycon, overridePost.
-        destruct (eq_dec ek EK_normal); [subst | apply drop_tc_environ].
-        Intros; unfold POSTCONDITION, abbreviate, normal_ret_assert, loop1_ret_assert, overridePost.
-        rewrite eq_dec_refl; entailer!.
+        entailer!.
       * forward.
         if_tac; [|contradiction].
         subst; entailer!.
-      * intros.
-        unfold exit_tycon, overridePost.
-        destruct (eq_dec ek EK_normal); [subst | apply drop_tc_environ].
-        Intros; unfold POSTCONDITION, abbreviate, normal_ret_assert, loop1_ret_assert, overridePost.
-        rewrite eq_dec_refl; entailer!.
+      * entailer!.
     + forward.
       subst; entailer!.
-    + forward; rewrite Hpi.
+    + forward; setoid_rewrite Hpi.
       { entailer!. }
-      forward_call (pvi, 0, v, P * ghost_snap k (Znth (i1 mod size) lg Vundef) *
-          fold_right sepcon emp (map (fun i => ghost_snap (Znth ((i + hash k) mod size) keys 0)
-            (Znth ((i + hash k) mod size) lg Vundef)) (upto (Z.to_nat i))),
-        II, lI, fun sh (v : Z) => !!(sh = Tsh) && EX H : _, EX T : _, !!(Zlength T = size /\ wf_table T /\
-          forall k v, H k = Some v <-> In (k, v) T /\ v <> 0) && let '(ki, vi) := Znth (i1 mod size) T (0, 0) in
-          !!(ki = k /\ vi = v /\ repable_signed vi) && ghost_master k (Znth (i1 mod size) lg Vundef) *
-          data_at Tsh tint (vint k) pki * ghost (Some H) g * fold_right sepcon emp (upd_Znth (i1 mod size)
+      forward_call (pvi, 0, v, |> P * (AS && emp) * ghost_snap k (Znth (i1 mod size) lg) *
+          fold_right sepcon emp (map (fun i => ghost_snap (Znth ((i + hash k) mod size) keys)
+            (Znth ((i + hash k) mod size) lg)) (upto (Z.to_nat i))) *
+          data_at sh (tarray tentry size) entries (gv _m_entries),
+        Full_set iname, Empty_set iname, fun sh1 (v1 : Z) => !!(sh1 = Tsh) && EX H : _, EX T : _, !!(Zlength T = size /\ wf_table T /\
+          forall k v, H k = Some v <-> In (k, v) T /\ v <> 0) && let '(ki, vi) := Znth (i1 mod size) T in
+          !!(ki = k /\ vi = v1 /\ repable_signed vi) && ghost_master1 k (Znth (i1 mod size) lg) *
+          data_at Tsh tint (vint k) pki * excl g H * fold_right sepcon emp (upd_Znth (i1 mod size)
             (map (hashtable_entry T lg entries) (upto (Z.to_nat size))) emp) *
-          R H * ghost_snap k (Znth (i1 mod size) lg Vundef) * fold_right sepcon emp (map (fun i =>
-            ghost_snap (Znth ((i + hash k) mod size) keys 0) (Znth ((i + hash k) mod size) lg Vundef)) (upto (Z.to_nat i))),
-        fun v => EX H' : _, Q H' (if eq_dec v 0 then true else false)).
-      { split; auto; split; auto; split.
-        + rewrite <- !sepcon_assoc, sepcon_assoc; etransitivity; [apply view_shift_sepcon1, HP|].
-          view_shift_intro HT.
-          unfold hashtable.
-          view_shift_intro T.
+          ghost_snap k (Znth (i1 mod size) lg) * fold_right sepcon emp (map (fun i =>
+            ghost_snap (Znth ((i + hash k) mod size) keys) (Znth ((i + hash k) mod size) lg)) (upto (Z.to_nat i))) *
+          data_at sh (tarray tentry size) entries (gv _m_entries) *
+          (ALL y : bool ,
+           weak_fview_shift (Empty_set iname) (Full_set iname)
+             (data_at sh (tarray tentry size) entries (gv _m_entries) *
+              (!! (H k = None <-> y = true) &&
+               hashtable (if y then map_upd H k v else H) g lg entries)) 
+             (Q y) && emp),
+        fun v => Q (if eq_dec v 0 then true else false)).
+      { cancel.
+        rewrite <- emp_sepcon, <- sepcon_emp at 1.
+        apply sepcon_derives; [|cancel].
+        apply sepcon_derives, derives_refl.
+        rewrite <- emp_sepcon at 1; apply sepcon_derives.
+        + unfold weak_fview_shift; rewrite <- wand_sepcon_adjoint, emp_sepcon.
+          rewrite (sepcon_comm _ (AS && emp)); unfold AS.
+          rewrite 2sepcon_assoc.
+          eapply derives_trans; [apply sepcon_derives, derives_refl; apply apply_fview_shift|].
+          eapply derives_trans; [apply fupd_frame_r | apply fupd_mono].
+          Intros HT.
+          unfold hashtable at 1; Intros T.
           rewrite extract_nth_sepcon with (i := i1 mod size)
             by (rewrite Zlength_map, Zlength_upto, Z2Nat.id; omega).
           erewrite Znth_map, Znth_upto by (rewrite ?Zlength_upto, Z2Nat.id; omega).
           unfold hashtable_entry.
           rewrite Hpi.
-          destruct (Znth (i1 mod size) T (0, 0)) as (ki, vi) eqn: HHi.
-          view_shift_intros.
-          rewrite <- !sepcon_assoc, (sepcon_comm _ (ghost_master _ _)).
+          destruct (Znth (i1 mod size) T) as (ki, vi) eqn: HHi; Intros.
+          rewrite <- !sepcon_assoc, (sepcon_comm _ (ghost_master1 _ _)).
           rewrite (sepcon_comm _ (ghost_snap _ _)), <- !sepcon_assoc.
-          rewrite snap_master_join1, !sepcon_andp_prop'; apply view_shift_prop; intro Hk1.
-          rewrite <- (prop_true_andp _ (ghost_master _ _) Hk1).
-          rewrite <- (@snap_master_join1 _ _ _ zero_order).
-          destruct Hk1; [contradiction | subst].
-          apply derives_view_shift.
+          rewrite snap_master_join1, !sepcon_andp_prop'; Intros.
+          rewrite <- (prop_true_andp _ (ghost_master1 _ _) H20).
+          rewrite <- (@snap_master_join1 _ _ zero_order).
+          destruct H20; [contradiction | subst].
+          rewrite (sepcon_comm _ (_ && _)), !sepcon_assoc.
+          eapply derives_trans; [apply sepcon_derives; [apply andp_left2|]; apply derives_refl|].
           Exists Tsh vi HT T; rewrite HHi; entailer!.
-        + intros.
-          view_shift_intro HT; view_shift_intro T.
-          etransitivity; [|etransitivity; [apply HQ | apply derives_view_shift; Exists HT; entailer!]].
-          destruct (Znth (i1 mod size) T (0, 0)) eqn: HHi.
-          view_shift_intros.
-          rewrite <- !sepcon_assoc, (sepcon_comm _ (ghost (Some HT) g)), !sepcon_assoc.
-          etransitivity; [apply view_shift_sepcon1|].
+          rewrite sepcon_comm; apply derives_refl.
+        + apply allp_right; intro sh0.
+          apply allp_right; intro v0.
+          unfold weak_fview_shift; rewrite <- wand_sepcon_adjoint, emp_sepcon.
+          Intros HT T.
+          destruct (Znth (i1 mod size) T) eqn: HHi; Intros.
+          rewrite <- !sepcon_assoc, (sepcon_comm _ (excl g HT)), !sepcon_assoc.
+          eapply derives_trans; [apply sepcon_derives, derives_refl|].
           { apply exclusive_update with (v' := if eq_dec v0 0 then map_upd HT k v else HT). }
-          apply derives_view_shift.
+          eapply derives_trans; [apply bupd_frame_r | apply fupd_bupd, bupd_mono].
+          rewrite <- !sepcon_assoc, sepcon_comm.
+          eapply derives_trans, apply_fview_shift'.
+          { apply sepcon_derives, derives_refl.
+            eapply allp_left, derives_refl. }
+          assert_PROP (lookup T k = Some (i1 mod size)) as Hindex.
+          { rewrite (sepcon_comm _ (fold_right _ _ _)), <- !sepcon_assoc,
+              (sepcon_comm _ (fold_right _ _ _)), <- !sepcon_assoc, 5sepcon_assoc.
+            apply sepcon_derives_prop, entries_lookup; auto.
+            rewrite HHi; auto. }
+          rewrite sepcon_comm, <- !sepcon_assoc, sepcon_assoc.
+          eapply derives_trans.
+          { apply sepcon_derives; [apply derives_refl|].
+            eapply derives_trans, bupd_sepcon.
+            apply sepcon_derives; [apply own_dealloc | apply snaps_dealloc]. }
+          eapply derives_trans; [apply bupd_frame_l | apply bupd_mono].
           unfold hashtable.
           Exists (if eq_dec v0 0 then upd_Znth (i1 mod size) T (k, v) else T).
           rewrite extract_nth_sepcon with (i := i1 mod size)(l := map _ (upto (Z.to_nat size)))
             by (rewrite Zlength_map, Zlength_upto, Z2Nat.id; omega).
           erewrite Znth_map, Znth_upto by (rewrite ?Zlength_upto, Z2Nat.id; omega).
-          assert_PROP (lookup T k = Some (i1 mod size)) as Hindex.
-          { pose proof (entries_lookup k i i1 keys lg T entries) as Hlookup.
-            subst; sep_apply Hlookup; rewrite ?HHi; auto.
-            apply sepcon_derives_prop; auto. }
           unfold hashtable_entry.
           if_tac; subst.
           * rewrite upd_Znth_same by omega.
@@ -1307,7 +1513,7 @@ Proof.
                 -- eapply In_upd_Znth_old; auto; try omega.
                    rewrite HHi; intro X; inv X; contradiction.
                 -- apply In_upd_Znth in Hin; destruct Hin as [X|]; [inv X; tauto | auto]. }
-            rewrite <- sepcon_emp, !sepcon_assoc; apply sepcon_derives.
+            apply sepcon_derives; [apply derives_refl|].
             apply sepcon_list_derives; rewrite !upd_Znth_Zlength;
               rewrite !Zlength_map, !Zlength_upto, !Z2Nat.id; auto; try omega.
             intros; destruct (eq_dec i0 (i1 mod size)).
@@ -1315,20 +1521,20 @@ Proof.
             rewrite !upd_Znth_diff' by (rewrite ?Zlength_map, ?Zlength_upto, ?Z2Nat.id; auto; omega).
             erewrite !Znth_map, !Znth_upto by (rewrite ?Zlength_upto, Z2Nat.id; auto; omega).
             rewrite upd_Znth_diff'; auto; omega.
-            { admit. (* drop snaps *) }
           * rewrite Hpi, HHi; entailer!.
             split; [|discriminate].
             assert (HT k = Some v0) as X; [|rewrite X; discriminate].
             match goal with H : forall k v, _ <-> _ |- _ => rewrite H end.
             split; auto; rewrite <- HHi; apply Znth_In; omega.
-            { admit. (* drop snaps *) } }
+            apply derives_refl. }
       unfold POSTCONDITION, abbreviate; simpl map.
-      Intros v' H'; forward.
-      Exists (if eq_dec v' 0 then true else false) H'; entailer!.
+      Intros v'; forward.
+      Exists (if eq_dec v' 0 then true else false); entailer!.
       if_tac; auto.
   - Intros i i1 keys.
     forward.
-    unfold loop2_ret_assert.
+    { entailer!.
+      rewrite (Int.signed_repr 1) by computable; omega. }
     Exists (i + 1) (i1 + 1) keys; entailer!.
     split.
     { rewrite <- Zplus_mod_idemp_l.
@@ -1344,59 +1550,61 @@ Proof.
   start_function.
   forward_for_simple_bound size (EX i : Z, EX entries : list (val * val),
     PROP (Forall (fun '(pk, pv) => isptr pk /\ isptr pv) entries; Zlength entries = i)
-    LOCAL (gvar _m_entries p)
-    SEP (@data_at CompSpecs Ews (tarray tentry size) (entries ++ repeat (Vundef, Vundef) (Z.to_nat (size - i))) p;
+    LOCAL (gvars gv)
+    SEP (@data_at CompSpecs Ews (tarray tentry size) (entries ++ repeat (Vundef, Vundef) (Z.to_nat (size - i))) (gv _m_entries);
          fold_right sepcon emp (map (fun x =>
-           malloc_token Tsh (sizeof tint) (fst x) * malloc_token Tsh (sizeof tint) (snd x)) entries);
-         EX lg : list val, !!(Zlength lg = i) && fold_right sepcon emp (map (fun j =>
+           malloc_token Tsh tint (fst x) * malloc_token Tsh tint (snd x)) entries);
+         EX lg : list gname, !!(Zlength lg = i) && fold_right sepcon emp (map (fun j =>
            hashtable_entry (repeat (0, 0) (Z.to_nat size)) lg entries j) (upto (Z.to_nat i))))).
-  { pose proof size_pos; split; [computable | omega]. }
+  { setoid_rewrite (proj2_sig has_size); reflexivity. }
+  { pose proof size_pos; omega. }
   { setoid_rewrite (proj2_sig has_size); computable. }
-  - go_lower.
-    Exists (@nil (val * val)) (@nil val); entailer!.
-    { setoid_rewrite (proj2_sig has_size); auto. }
+  - Exists (@nil (val * val)) (@nil gname); entailer!.
     rewrite data_at__eq; unfold default_val; simpl.
-    rewrite repeat_list_repeat, Z.sub_0_r; auto.
+    rewrite repeat_list_repeat, Z.sub_0_r; apply derives_refl.
   - Intros lg.
-    eapply ghost_alloc with (g := (Tsh, 0)); auto with init.
+    ghost_alloc (ghost_master1 0).
     Intros gk.
-    forward_malloc tint pk.
+    forward_call tint.
+    { split; auto; simpl; computable. }
+    Intros pk.
     rewrite sepcon_map; Intros.
     repeat forward.
-    forward_malloc tint pv.
+    forward_call tint.
+    { split; auto; simpl; computable. }
+    Intros pv.
     repeat forward.
-    assert (0 <= i < Zlength (x ++ repeat (Vundef, Vundef) (Z.to_nat (size - i)))).
+    assert (0 <= i < Zlength (entries ++ repeat (Vundef, Vundef) (Z.to_nat (size - i)))).
     { rewrite Zlength_app, Zlength_repeat, Z2Nat.id; omega. }
     rewrite upd_Znth_twice, upd_Znth_same by auto.
-    go_lower; Exists (x ++ [(pk, pv)]) (lg ++ [gk]).
+    go_lower; Exists (entries ++ [(pk, pv)]) (lg ++ [gk]).
     rewrite !Z2Nat.inj_add, !upto_app, !map_app, !sepcon_app, !Z2Nat.id by omega.
     change (upto (Z.to_nat 1)) with [0]; unfold hashtable_entry at 3; simpl.
     rewrite Z.add_0_r, !app_Znth2 by omega.
-    replace (Zlength x) with i; replace (Zlength lg) with i; rewrite Zminus_diag, !Znth_0_cons.
-    rewrite Znth_repeat, !Zlength_app, !Zlength_cons, !Zlength_nil; entailer!.
-    { split; [setoid_rewrite (proj2_sig has_size); auto|].
-      rewrite Forall_app; repeat constructor; auto. }
-    rewrite upd_init, <- app_assoc by (auto; omega); unfold ghost_master; cancel.
+    replace (Zlength entries) with i; replace (Zlength lg) with i; rewrite Zminus_diag, !Znth_0_cons.
+    rewrite Znth_repeat', !Zlength_app, !Zlength_cons, !Zlength_nil by (rewrite Z2Nat.id; omega).
+    entailer!.
+    { rewrite Forall_app; repeat constructor; auto. }
+    rewrite upd_init, <- app_assoc by (auto; omega); cancel.
     rewrite <- sepcon_map; cancel.
     apply sepcon_list_derives; rewrite !Zlength_map, !Zlength_upto; auto.
     rewrite <- Zlength_correct; intros.
     erewrite !Znth_map, !Znth_upto by (rewrite ?Zlength_upto, <- Zlength_correct; auto; omega).
-    unfold hashtable_entry; rewrite !app_Znth1 by omega; auto.
+    unfold hashtable_entry; rewrite !app_Znth1 by omega; apply derives_refl.
   - Intros entries lg.
     rewrite Zminus_diag, app_nil_r.
-    eapply (@ghost_alloc _ _ exclusive_PCM (Some (fun _ => None))).
-    { exists None; exists (Some (fun _ : Z => @None Z)); simpl; auto. }
+    ghost_alloc (fun g => excl g (@empty_map Z Z)).
     Intro g.
     forward.
     unfold hashtable; Exists entries g lg (repeat (0, 0) (Z.to_nat size)); entailer!.
     split; [rewrite Zlength_repeat, Z2Nat.id; auto; pose proof size_pos; omega|].
     split.
     + intros ??? Hj.
-      rewrite Znth_repeat in Hj; simpl in Hj; subst; contradiction.
+      setoid_rewrite Znth_repeat in Hj; simpl in Hj; subst; contradiction.
     + split; [discriminate|].
       intros (Hin & ?); apply repeat_spec in Hin; inv Hin; contradiction.
-    + unfold empty_map; cancel.
-      erewrite map_ext; eauto; intros (?, ?); auto.
+    + apply sepcon_derives; erewrite map_ext; try apply derives_refl; auto.
+      intros (?, ?); auto.
 Qed.
 
 Lemma lock_struct_array : forall sh z (v : list val) p,
@@ -1405,34 +1613,38 @@ Lemma lock_struct_array : forall sh z (v : list val) p,
 Proof.
   intros.
   unfold data_at, field_at, at_offset; rewrite !data_at_rec_eq; simpl; f_equal.
+  f_equal.
+  apply prop_ext; split; intros (? & ? & ? & Halign & ?); repeat split; auto.
+  - destruct p; try contradiction; simpl in *.
+    inv Halign; try discriminate.
+    constructor; auto.
+    intros ? Hi; specialize (H7 _ Hi).
+    inv H7; econstructor; eauto.
+  - destruct p; try contradiction; simpl in *.
+    inv Halign; try discriminate.
+    constructor; auto.
+    intros ? Hi; specialize (H7 _ Hi).
+    inv H7; econstructor; eauto.
 Qed.
 
-Lemma f_pred_precise : forall tsh sh gsh (entries : list (val * val)) gh g lg p t locksp lockt resultsp res,
+Lemma f_pred_exclusive : forall tsh sh gsh (entries : list (val * val)) i gh g lg p t locksp lockt resultsp res,
   readable_share sh -> Zlength lg = Zlength entries ->
-  precise (f_lock_pred tsh sh gsh entries gh g lg p t locksp lockt resultsp res).
+  exclusive_mpred (f_lock_pred tsh sh gsh entries i gh g lg p t locksp lockt resultsp res).
 Proof.
   intros; unfold f_lock_pred.
-  apply selflock_precise.
+  apply selflock_exclusive.
   unfold f_lock_inv.
-  eapply derives_precise' with (Q := (EX g : option (share * hist) * option hist, ghost g gh) *
-    data_at_ _ _ _ * invariant (hashtable_inv gh g lg entries) *
-    data_at_ sh _ _ * data_at_ _ _ _ * data_at_ _ _ _).
-  - Intros b1 b2 b3 h.
-    repeat (apply sepcon_derives; try apply data_at_data_at_).
-    + unfold ghost_hist.
-      Exists (Some (gsh, h), @None hist); auto.
-    + auto.
-  - repeat (apply precise_sepcon; auto).
-    + apply ex_ghost_precise.
-    + apply invariant_precise.
+  eapply derives_exclusive, exclusive_sepcon1 with
+    (P := @data_at CompSpecs sh (tarray tentry size) entries p)(Q := EX b1 : bool, EX b2 : bool,
+    EX b3 : bool, EX h : nat -> option hashtable_hist_el, _), data_at_exclusive; auto.
+  - Intros b1 b2 b3 h; Exists b1 b2 b3 h.
+    rewrite (sepcon_comm (ghost_hist _ _ _)), !sepcon_assoc.
+    apply sepcon_derives; auto.
+  - simpl.
+    pose proof size_pos.
+    rewrite Z.max_r; omega.
 Qed.
-
-Lemma f_pred_positive : forall tsh sh gsh entries gh g lg p t locksp lockt resultsp res,
-  positive_mpred (f_lock_pred tsh sh gsh entries gh g lg p t locksp lockt resultsp res).
-Proof.
-  intros; apply selflock_positive.
-Qed.
-Hint Resolve f_pred_precise f_pred_positive.
+Hint Resolve f_pred_exclusive.
 
 Lemma apply_hist_app : forall h1 h2 H, apply_hist H (h1 ++ h2) =
   match apply_hist H h1 with Some H' => apply_hist H' h2 | None => None end.
@@ -1440,16 +1652,13 @@ Proof.
   induction h1; auto; simpl; intros.
   destruct a; rewrite IHh1; auto.
   - destruct (H k); if_tac; auto.
-  - destruct (H k); if_tac; auto.
+  - destruct (H k); simple_if_tac; auto.
 Qed.
 
 Lemma body_f : semax_body Vprog Gprog f_f f_spec.
 Proof.
   start_function.
   rewrite (data_at_isptr Tsh); Intros.
-  assert (force_val (sem_cast_neutral tid) = tid) as Htid.
-  { destruct tid; try contradiction; auto. }
-  focus_SEP 3.
   forward.
   rewrite <- lock_struct_array.
   forward.
@@ -1460,26 +1669,57 @@ Proof.
     rewrite upd_Znth_same; auto. }
   rewrite !upd_Znth_same by auto.
   forward.
-  forward_call (tid, sizeof tint).
-  { rewrite !sepcon_assoc; apply sepcon_derives; [apply data_at_memory_block | cancel_frame]. }
-  forward_for_simple_bound 3 (EX i : Z, EX ls : list bool,
-    PROP (Zlength ls = i)
+  forward_call (tint, tid).
+  forward_for_simple_bound 3 (EX j : Z, EX ls : list bool, EX h : _,
+    PROP (Zlength ls = j; add_events empty_map (map (fun j => HAdd (j + 1) 1 (Znth j ls)) (upto (Z.to_nat j))) h)
     LOCAL (temp _total (vint (Zlength (filter id ls))); temp _res res; temp _l lockt; temp _t (vint t);
-           temp _arg tid; gvar _m_entries p; gvar _thread_locks locksp; gvar _results resultsp)
-    SEP (@data_at CompSpecs sh (tarray tentry size) entries p; invariant (hashtable_inv gh g lg entries);
-         EX h : _, !!(add_events [] (map (fun j => HAdd (j + 1) 1 (Znth j ls false)) (upto (Z.to_nat i))) h) &&
-           ghost_hist gsh h gh;
-         data_at sh (tarray (tptr (Tstruct _lock_t noattr)) 3) (upd_Znth t (repeat Vundef 3) lockt) locksp;
-         data_at sh (tarray (tptr tint) 3) (upd_Znth t (repeat Vundef 3) res) resultsp;
+           temp _arg tid; gvars gv)
+    SEP (@data_at CompSpecs sh (tarray tentry size) entries (gv _m_entries); invariant i (hashtable_inv gh g lg entries);
+         ghost_hist gsh h gh;
+         data_at sh (tarray (tptr (Tstruct _lock_t noattr)) 3) (upd_Znth t (repeat Vundef 3) lockt) (gv _thread_locks);
+         data_at sh (tarray (tptr tint) 3) (upd_Znth t (repeat Vundef 3) res) (gv _results);
          data_at_ Tsh tint res;
-         lock_inv tsh lockt (f_lock_pred tsh sh gsh entries gh g lg p t locksp lockt resultsp res))).
-  - Exists (@nil bool) (@nil (nat * hashtable_hist_el)); entailer!.
-  - Intros h.
-    forward_call (i + 1, 1, p, sh, entries, g, lg, ghost_hist gsh h gh,
-      fun (_ : Z -> option Z) b => EX h' : _, !!(add_events h [HAdd (i + 1) 1 b] h') && ghost_hist gsh h' gh,
-      fun H => ghost_hist gsh h gh * EX hr : _, !!(apply_hist empty_map hr = Some H) && ghost_ref hr gh,
-      fun p : Z => hashtable_inv gh g lg entries, [0]).
+         lock_inv tsh lockt (f_lock_pred tsh sh gsh entries i gh g lg (gv _m_entries) t
+                                         (gv _thread_locks) lockt (gv _results) res))).
+  - Exists (@nil bool) (@empty_map nat hashtable_hist_el); entailer!.
+  - forward_call (i0 + 1, 1, gv, sh, entries, g, lg,
+      fun b => EX h' : _, !!(add_events h [HAdd (i0 + 1) 1 b] h') && ghost_hist gsh h' gh).
     { simpl; entailer!.
+      { match goal with H : Forall (fun '(pk, pv) => isptr pk /\ isptr pv) entries |- _ =>
+          eapply Forall_impl, H end; intros (?, ?); auto. }
+      unfold atomic_shift.
+      Print corable.corable.
+      Locate "|>".
+      Locate boox.
+      Check boxedE.
+      Print predicates_hered.laterM.
+      Print ageable.laterR.
+      Check boxE.
+      Exists (invariant i (hashtable_inv gh g lg entries) * ghost_hist gsh h gh *
+        data_at sh (tarray (tptr tint) 3) (upd_Znth t [Vundef; Vundef; Vundef] res) (gv _results)).
+      rewrite !sepcon_assoc.
+      eapply derives_trans, sepcon_derives, derives_refl; [|apply now_later].
+      cancel.
+      rewrite <- emp_sepcon at 1; apply sepcon_derives; [|cancel].
+      apply andp_right; auto.
+      unfold weak_fview_shift; rewrite <- wand_sepcon_adjoint, emp_sepcon.
+      rewrite 2later_sepcon at 1.
+      eapply derives_trans.
+      { apply sepcon_derives, sepcon_derives, derives_refl; apply except0_timeless;
+          try apply except0_intro.
+
+  rewrite <- later_exp.
+
+        admit.
+        admit. }
+        + 
+      SearchAbout timeless later.
+      
+      Check inv_open.
+      apply 
+      
+      
+      SearchAbout fupd.
       split; [split|].
       + pose proof (Int.min_signed_neg); omega.
       + transitivity 4; [omega | computable].
@@ -1527,31 +1767,31 @@ Proof.
       rewrite In_upto, Z2Nat.id in Hj; omega.
   - Intros ls h.
     forward.
-    forward_call (lockt, tsh, f_lock_inv sh gsh entries gh g lg p t locksp lockt resultsp res,
-                  f_lock_pred tsh sh gsh entries gh g lg p t locksp lockt resultsp res).
+    forward_call (lockt, tsh, f_lock_inv sh gsh entries i gh g lg (gv _m_entries) t
+      (gv _thread_locks) lockt (gv _results) res,
+                  f_lock_pred tsh sh gsh entries i gh g lg (gv _m_entries) t
+      (gv _thread_locks) lockt (gv _results) res).
     { assert_PROP (Zlength entries = size) by (pose proof size_pos; entailer!).
       lock_props.
-      { apply f_pred_precise; auto; omega. }
-      { apply selflock_rec. }
       unfold f_lock_pred at 2.
       rewrite selflock_eq.
       unfold f_lock_inv at 1.
       rewrite lock_struct_array.
-      Exists (Znth 0 ls false) (Znth 1 ls false) (Znth 2 ls false) h; entailer!.
-      rewrite (list_Znth_eq false ls) at 1.
+      Exists (Znth 0 ls) (Znth 1 ls) (Znth 2 ls) h; entailer!.
+      rewrite (list_Znth_eq ls) at 1.
       replace (length ls) with (Z.to_nat 3) by (symmetry; rewrite <- Zlength_length by computable; auto).
       cancel.
       subst Frame; instantiate (1 := []); simpl; rewrite sepcon_emp; apply lock_inv_later. }
     forward.
 Qed.
 
-Lemma lock_struct : forall p, data_at_ Tsh (Tstruct _lock_t noattr) p |-- data_at_ Tsh tlock p.
+(*Lemma lock_struct : forall p, data_at_ Tsh (Tstruct _lock_t noattr) p |-- data_at_ Tsh tlock p.
 Proof.
   intros.
   unfold data_at_, field_at_; unfold_field_at 1%nat.
   unfold field_at, at_offset; simpl.
   rewrite field_compatible_cons; simpl; entailer!.
-Qed.
+Qed.*)
 
 Lemma add_fails : forall k v b l H H' (HH : apply_hist H l = Some H') (Hadd : In (HAdd k v b) l)
   (Hk : H k <> None), b = false.
@@ -1568,14 +1808,14 @@ Proof.
 Qed.
 
 Lemma only_one_add_succeeds : forall k v1 v2 l i1 i2 H0 H (HH : apply_hist H0 l = Some H)
-  (Hin1 : Znth i1 l (HGet 0 0) = HAdd k v1 true) (Hin2 : Znth i2 l (HGet 0 0) = HAdd k v2 true),
+  (Hin1 : Znth i1 l = HAdd k v1 true) (Hin2 : Znth i2 l = HAdd k v2 true),
   i2 = i1 /\ v2 = v1.
 Proof.
   induction l; simpl; intros.
   { rewrite Znth_nil in Hin1; discriminate. }
   assert (i2 = i1); [|subst; rewrite Hin2 in Hin1; inv Hin1; auto].
-  exploit (Znth_inbounds i1 (a :: l) (HGet 0 0)); [rewrite Hin1; discriminate|].
-  exploit (Znth_inbounds i2 (a :: l) (HGet 0 0)); [rewrite Hin2; discriminate|].
+  exploit (Znth_inbounds i1 (a :: l)); [rewrite Hin1; discriminate|].
+  exploit (Znth_inbounds i2 (a :: l)); [rewrite Hin2; discriminate|].
   rewrite !Zlength_cons; intros.
   destruct (eq_dec i1 0), (eq_dec i2 0); subst; auto.
   - rewrite Znth_0_cons in Hin1; subst.
@@ -1616,8 +1856,8 @@ Proof.
       unfold map_upd; if_tac; auto; subst; contradiction.
 Qed.
 
-Lemma filter_find_count : forall {A} (f : A -> bool) d l li (Hunique : NoDup li)
-  (Hli : forall i, In i li -> f (Znth i l d) = true) (Hrest : forall i, ~In i li -> f (Znth i l d) = false),
+Lemma filter_find_count : forall {A} {d : Inhabitant A} (f : A -> bool) l li (Hunique : NoDup li)
+  (Hli : forall i, In i li -> f (Znth i l) = true) (Hrest : forall i, ~In i li -> f (Znth i l) = false),
   Zlength (filter f l) = Zlength li.
 Proof.
   induction l; simpl; intros.
@@ -1679,17 +1919,17 @@ Proof.
         contradiction Hj; rewrite in_map_iff; do 2 eexists; eauto; omega.
 Qed.
 
-Lemma hists_eq : forall lr (Hlr : Forall (fun '(h, ls) => add_events []
-  [HAdd 1 1 (Znth 0 ls false); HAdd 2 1 (Znth 1 ls false); HAdd 3 1 (Znth 2 ls false)] h) lr)
+Lemma hists_eq : forall lr (Hlr : Forall (fun '(h, ls) => add_events empty_map
+  [HAdd 1 1 (Znth 0 ls); HAdd 2 1 (Znth 1 ls); HAdd 3 1 (Znth 2 ls)] h) lr)
   (Hlens : Forall (fun '(_, ls) => Zlength ls = 3) lr),
   map snd lr = map (fun x => map (fun e => match snd e with | HAdd _ _ b => b | _ => false end) (fst x)) lr.
 Proof.
   intros; apply list_Znth_eq' with (d := []); rewrite !Zlength_map; auto.
   intros.
-  rewrite !Znth_map with (d' := ([], [])) by auto.
-  apply Forall_Znth with (i := j)(d := ([], [])) in Hlr; auto.
-  apply Forall_Znth with (i := j)(d := ([], [])) in Hlens; auto.
-  destruct (Znth j lr ([], [])); simpl.
+  rewrite !Znth_map) by auto.
+  apply Forall_Znth with (i := j)) in Hlr; auto.
+  apply Forall_Znth with (i := j)) in Hlens; auto.
+  destruct (Znth j lr); simpl.
   apply add_events_add in Hlr; destruct Hlr as (l' & ? & Heq); subst.
   destruct l0; [discriminate | rewrite Zlength_cons in *].
   destruct l0; [discriminate | rewrite Zlength_cons in *].
@@ -1702,8 +1942,8 @@ Proof.
 Qed.
 
 Lemma add_three : forall lr HT l (Hlr : Zlength lr = 3)
-  (Hhists : Forall (fun '(h, ls) => add_events [] [HAdd 1 1 (Znth 0 ls false); HAdd 2 1 (Znth 1 ls false);
-     HAdd 3 1 (Znth 2 ls false)] h) lr) (Hlens : Forall (fun '(_, ls) => Zlength ls = 3) lr)
+  (Hhists : Forall (fun '(h, ls) => add_events empty_map [HAdd 1 1 (Znth 0 ls); HAdd 2 1 (Znth 1 ls);
+     HAdd 3 1 (Znth 2 ls)] h) lr) (Hlens : Forall (fun '(_, ls) => Zlength ls = 3) lr)
   (Hl : hist_list (concat (map fst lr)) l) (HHT : apply_hist empty_map l = Some HT),
   Zlength (filter id (concat (map snd lr))) = 3.
 Proof.
@@ -1725,15 +1965,15 @@ Proof.
     rewrite Forall_forall in Hhists; specialize (Hhists _ Hin); simpl in Hhists.
     erewrite add_events_snd in Hin' by eauto; simpl in Hin'.
     decompose [or] Hin'; try discriminate; contradiction. }
-  assert (forall i, 0 <= i < 3 -> In (HAdd (i + 1) 1 (Znth i (snd (Znth 0 lr ([], []))) false)) l) as Hins.
+  assert (forall i, 0 <= i < 3 -> In (HAdd (i + 1) 1 (Znth i (snd (Znth 0 lr )))) l) as Hins.
   { intros.
-    assert (exists t, In (t, HAdd (i + 1) 1 (Znth i (snd (Znth 0 lr ([], []))) false)) (concat (map fst lr)))
+    assert (exists t, In (t, HAdd (i + 1) 1 (Znth i (snd (Znth 0 lr)))) (concat (map fst lr)))
       as (t & Hin).
     { setoid_rewrite in_concat; setoid_rewrite in_map_iff.
       exploit (Znth_In 0 lr ([], [])); [omega | intro Hin].
       rewrite Forall_forall in Hhists; specialize (Hhists _ Hin).
       destruct (Znth 0 lr ([], [])) as (h, ?); simpl in *.
-      exploit (Znth_In i (map snd h) (HGet 0 0)).
+      exploit (Znth_In i (map snd h)).
       { erewrite add_events_snd; eauto; simpl.
         rewrite !Zlength_cons, Zlength_nil; auto. }
       intro Hin'; rewrite in_map_iff in Hin'; destruct Hin' as ((t, ?) & ? & Hin'); simpl in *; subst.
@@ -1795,10 +2035,11 @@ Proof.
   start_function.
   replace 16384 with size by (setoid_rewrite (proj2_sig has_size); auto).
   forward.
-  forward_call m_entries.
+  forward_call gv.
   { fast_cancel. }
   Intros x; destruct x as ((entries, g), lg).
-  apply ghost_alloc with (g0 := (Some (Tsh, [] : hist), Some ([] : hist))); auto with init.
+  ghost_alloc (ghost_hist_ref(hist_el := hashtable_hist_el) Tsh empty_map empty_map).
+  { split; auto; apply self_completable. }
   Intro gh.
   rewrite <- hist_ref_join_nil by (apply Share.nontrivial); Intros.
   gather_SEP 4 1; apply make_inv with (Q := hashtable_inv gh g lg entries).
@@ -2099,3 +2340,5 @@ Proof.
   rewrite <- (proj2_sig has_size).
   entailer!.
 Qed.
+
+End Proofs.
